theories/CertiGC/vst/proof/verif_forward.v
@@ -39,9 +39,8 @@ Qed.
 
 Lemma sapi_ptr_val: forall p m n,
     isptr p -> Int.min_signed <= n <= Int.max_signed ->
-    (force_val
-       (sem_add_ptr_int int_or_ptr_type Signed (offset_val (WORD_SIZE * m) p)
-                        (vint n))) = offset_val (WORD_SIZE * (m + n)) p.
+    (force_val (sem_add_ptr_int int_or_ptr_type Signed (offset_val (WORD_SIZE * m) p) (vint n)))
+    = offset_val (WORD_SIZE * (m + n)) p.
 Proof.
   intros. rewrite sem_add_pi_ptr_special; [| easy | | easy].
   - simpl. rewrite offset_offset_val. f_equal. fold WORD_SIZE; rep_lia.
@@ -51,13 +50,11 @@ Qed.
 Lemma sapil_ptr_val: forall p m n,
     isptr p ->
     if Archi.ptr64 then
-      force_val
-        (sem_add_ptr_long int_or_ptr_type (offset_val (WORD_SIZE * m) p)
-                          (Vlong (Int64.repr n))) = offset_val (WORD_SIZE * (m + n)) p
+      force_val (sem_add_ptr_long int_or_ptr_type (offset_val (WORD_SIZE * m) p) (Vlong (Int64.repr n)))
+      = offset_val (WORD_SIZE * (m + n)) p
     else
-      force_val
-        (sem_add_ptr_int int_or_ptr_type Signed (offset_val (WORD_SIZE * m) p)
-                         (vint n)) = offset_val (WORD_SIZE * (m + n)) p.
+      force_val (sem_add_ptr_int int_or_ptr_type Signed (offset_val (WORD_SIZE * m) p) (vint n))
+      = offset_val (WORD_SIZE * (m + n)) p.
 Proof.
   intros. simpl.
   first [rewrite sem_add_pi_ptr_special' | rewrite sem_add_pl_ptr_special']; auto.
@@ -68,10 +65,8 @@ Lemma data_at_mfs_eq: forall g v i sh nv,
     field_compatible int_or_ptr_type [] (offset_val (WORD_SIZE * i) nv) ->
     0 <= i < Zlength (block_fields (heapgraph_block g v)) ->
     data_at sh (tarray int_or_ptr_type i) (sublist 0 i (heapgraph_block_cells_vals g v)) nv *
-    field_at sh int_or_ptr_type [] (Znth i (heapgraph_block_cells_vals g v))
-             (offset_val (WORD_SIZE * i) nv) =
-    data_at sh (tarray int_or_ptr_type (i + 1))
-            (sublist 0 (i + 1) (heapgraph_block_cells_vals g v)) nv.
+    field_at sh int_or_ptr_type [] (Znth i (heapgraph_block_cells_vals g v)) (offset_val (WORD_SIZE * i) nv)
+    = data_at sh (tarray int_or_ptr_type (i + 1)) (sublist 0 (i + 1) (heapgraph_block_cells_vals g v)) nv.
 Proof.
   intros. rewrite field_at_data_at. unfold field_address.
   rewrite if_true by assumption. simpl nested_field_type.
@@ -81,7 +76,8 @@ Proof.
                 sh int_or_ptr_type _ [Znth i (heapgraph_block_cells_vals g v)]) by reflexivity.
   rewrite <- fields_eq_length in H0.
   rewrite (data_at_tarray_value
-             sh (i + 1) i nv (sublist 0 (i + 1) (heapgraph_block_cells_vals g v))
+             sh (i + 1) i nv
+             (sublist 0 (i + 1) (heapgraph_block_cells_vals g v))
              (heapgraph_block_cells_vals g v) (sublist 0 i (heapgraph_block_cells_vals g v))
              [Znth i (heapgraph_block_cells_vals g v)]).
   - replace (i + 1 - i) with 1 by lia. reflexivity.
@@ -112,87 +108,165 @@ Qed.
 Lemma body_forward: semax_body Vprog Gprog f_forward forward_spec.
 Proof.
   start_function.
-  destruct H as [? [? [? ?]]]. destruct H1 as [? [? [? [? ?]]]].
-  unfold limit_address, next_address, forward_p_address. destruct forward_p.
-  - unfold thread_info_rep. Intros.
-    assert (Zlength roots = Zlength (live_roots_indices f_info)) by
-        (rewrite <- (Zlength_map _ _ ((fun x y => Znth y x) (ti_args t_info))), <- H4, Zlength_map; trivial).
-    pose proof (Znth_map _ (root2val g) _ H0). hnf in H0. rewrite H11 in H0.
+  destruct H as [H [H4 [H5 H6]]].
+  destruct H1 as [H1 [H7 [H8 [H9 H10]]]].
+  unfold limit_address, next_address, forward_p_address.
+  destruct forward_p.
+  {
+    unfold thread_info_rep.
+    Intros.
+    assert
+      (Zlength roots = Zlength (live_roots_indices f_info))
+      as H11
+      by (rewrite <- (Zlength_map _ _ ((fun x y => Znth y x) (ti_args t_info))), <- H4, Zlength_map; trivial).
+    pose proof (Znth_map _ (root2val g) _ H0) as H12.
+    hnf in H0.
+    rewrite H11 in H0.
     rewrite H4, Znth_map in H12 by assumption.
-    remember (Znth z roots) as root. rewrite <- H11 in H0.
-    pose proof (Znth_In _ _ H0).
-    rewrite <- Heqroot in H13. rewrite H11 in H0. unfold Inhabitant_val in H12.
-    assert (forall v, In (inr v) roots -> isptr (heapgraph_block_ptr g v)). { (**)
-      intros. destruct H5. unfold heapgraph_block_ptr. red in H15.
+    remember
+      (Znth z roots)
+      as root eqn:Heqroot.
+    rewrite <- H11 in H0.
+    pose proof (Znth_In _ _ H0) as H13.
+    rewrite <- Heqroot in H13.
+    rewrite H11 in H0.
+    unfold Inhabitant_val in H12.
+    assert
+      (forall v, In (inr v) roots -> isptr (heapgraph_block_ptr g v))
+      as H14.
+    {
+      intros.
+      destruct H5 as [H5 H15].
+      unfold heapgraph_block_ptr.
+      red in H15.
       rewrite Forall_forall in H15.
-      rewrite (filter_sum_right_In_iff v roots) in H14. apply H15 in H14.
+      rewrite (filter_sum_right_In_iff v roots) in H14.
+      apply H15 in H14.
       pose proof (heapgraph_has_block__has_gen H14) as Hgen.
       apply heapgraph_generation_base__isptr in Hgen.
       remember (heapgraph_generation_base g (addr_gen v)) as vv.
-      destruct vv; try contradiction.
-      simpl. exact I.
+      now destruct vv.
     }
-    assert (is_pointer_or_integer (root2val g root)). {
+    assert
+      (is_pointer_or_integer (root2val g root))
+      as H15.
+    {
       destruct root as [[? | ?] | ?]; simpl; auto.
-      - destruct g0. simpl. exact I.
-      - specialize (H14 _ H13). apply isptr_is_pointer_or_integer. assumption. }
-    assert (0 <= Znth z (live_roots_indices f_info) < MAX_ARGS) by
-        (apply (fi_index_range f_info), Znth_In; assumption).
-    forward; rewrite H12. 1: entailer!.
-    assert_PROP (valid_int_or_ptr (root2val g root)). {
-      gather_SEP (graph_rep _) (outlier_rep _).
-      sep_apply (root_valid_int_or_ptr _ _ _ _ H13 H5). entailer!. }
-    forward_call (root2val g root).
-    remember (graph_rep g * heap_rest_rep (ti_heap t_info) * outlier_rep outlier)
-      as P. pose proof (graph_and_heap_rest_data_at_ _ _ _ H7 H).
-    unfold generation_data_at_ in H18. remember (heapgraph_generation_base g from) as fp.
-    remember (heapgraph_generation_sh g from) as fsh. remember (gen_size t_info from) as gn.
-    remember (WORD_SIZE * gn)%Z as fn.
-    assert (P |-- (weak_derives P (memory_block fsh fn fp * TT) && emp) * P). {
-      apply weak_derives_strong. subst. sep_apply H18.
-      rewrite data_at__memory_block.
-      rewrite sizeof_tarray_int_or_ptr; [Intros; cancel | unfold gen_size].
-      destruct (space_capacity__tight_range (nth_space t_info from)). assumption. }
-    destruct root as [[? | ?] | ?]; simpl root2val.
-    + unfold odd_Z2val. forward_if.
-      1: exfalso; apply H20'; reflexivity.
-      forward. Exists g t_info roots.
+      - now destruct g0.
+      - specialize (H14 _ H13).
+        now apply isptr_is_pointer_or_integer.
+    }
+    assert
+      (0 <= Znth z (live_roots_indices f_info) < MAX_ARGS)
+      as H16
+      by (apply (fi_index_range f_info), Znth_In; assumption).
+    forward; rewrite H12.
+    {
       entailer!.
-      * simpl; split3; try rewrite <- Heqroot; [easy..|].
+    }
+    assert_PROP
+      (valid_int_or_ptr (root2val g root))
+      as H17.
+    {
+      gather_SEP (graph_rep _) (outlier_rep _).
+      sep_apply (root_valid_int_or_ptr _ _ _ _ H13 H5).
+      entailer!.
+    }
+    forward_call (root2val g root).
+    remember
+      (graph_rep g * heap_rest_rep (ti_heap t_info) * outlier_rep outlier)
+      as P eqn:HeqP.
+    pose proof (graph_and_heap_rest_data_at_ _ _ _ H7 H) as H18.
+    unfold generation_data_at_ in H18.
+    remember
+      (heapgraph_generation_base g from)
+      as fp eqn:Heqfp.
+    remember
+      (heapgraph_generation_sh g from) as fsh.
+    remember
+      (gen_size t_info from - space_remembered (nth_space t_info from))
+      as gn eqn:Heqgn.
+    remember
+      (WORD_SIZE * gn)%Z
+      as fn eqn:Heqfn.
+    assert (P |-- (weak_derives P (memory_block fsh fn fp * TT) && emp) * P) as H19.
+    {
+      apply weak_derives_strong.
+      subst.
+      sep_apply H18.
+      unfold gen_size.
+      rewrite data_at__memory_block.
+      pose proof (space_remembered__order (nth_space t_info from)) as H19.
+      rewrite sizeof_tarray_int_or_ptr ; try lia.
+      entailer!.
+    }
+    destruct root as [[? | ?] | ?]; simpl root2val.
+    {
+      unfold odd_Z2val.
+      forward_if.
+      {
+        exfalso.
+        now apply H20'.
+      }
+      forward.
+      Exists g t_info roots.
+      entailer!.
+      - simpl; split3; try rewrite <- Heqroot; [easy..|].
         split3; [constructor | easy | apply tir_id].
-      * unfold thread_info_rep. entailer!.
-    + unfold GC_Pointer2val. destruct g0. forward_if.
-      2: exfalso; apply Int.one_not_zero in H20; assumption.
+      - unfold thread_info_rep.
+        entailer!.
+    }
+    {
+      unfold GC_Pointer2val.
+      destruct g0.
+      forward_if.
+      2: {
+        exfalso.
+        now apply Int.one_not_zero in H20.
+      }
       forward_call (Vptr b i).
       gather_SEP (graph_rep _) (heap_rest_rep _) (outlier_rep _).
-      rewrite <- HeqP. destruct H5.
-      replace_SEP 0 ((weak_derives P (memory_block fsh fn fp * TT) && emp) * P) by
-          (entailer; assumption). clear H19. Intros. simpl root2val in *.
-      assert (P |-- (weak_derives P (valid_pointer (Vptr b i) * TT) && emp) * P). {
+      rewrite <- HeqP.
+      destruct H5 as [H5 H21].
+      replace_SEP 0
+        ((weak_derives P (memory_block fsh fn fp * TT) && emp) * P)
+        by (entailer; assumption).
+      clear H19.
+      Intros.
+      simpl root2val in *.
+      assert
+        (P |-- (weak_derives P (valid_pointer (Vptr b i) * TT) && emp) * P)
+        as H19.
+      {
         subst. cancel. apply andp_right. 2: cancel.
         assert (HS: emp |-- TT) by entailer; sep_apply HS; clear HS.
         apply derives_weak.
         sep_apply (roots_outlier_rep_valid_pointer _ _ _ H13 H5).
-        simpl GC_Pointer2val. cancel. }
-      replace_SEP 1 ((weak_derives P (valid_pointer (Vptr b i) * TT) && emp) * P) by
-          (entailer; assumption). Intros. clear H19.
-      forward_call (fsh, fp, fn, (Vptr b i), P).
-      {
-        entailer!.
-        simpl.
-        f_equal.
-        admit.
+        simpl GC_Pointer2val. cancel.
       }
-      Intros v. destruct v.
+      replace_SEP 1
+        ((weak_derives P (valid_pointer (Vptr b i) * TT) && emp) * P)
+        by (entailer; assumption).
+      Intros.
+      clear H19.
+      forward_call (fsh, fp, fn, (Vptr b i), P).
+      Intros v.
+      destruct v.
       * rewrite HeqP. Intros.
         gather_SEP (graph_rep g) (heap_rest_rep _).
-        sep_apply H18. rewrite Heqfn in v.
-        sep_apply (roots_outlier_rep_single_rep _ _ _ H13 H5). Intros.
+        sep_apply H18.
+        rewrite Heqfn in v.
+        sep_apply (roots_outlier_rep_single_rep _ _ _ H13 H5).
+        Intros.
         gather_SEP (single_outlier_rep _) (data_at_ _ _ _).
         change (Vptr b i) with (GC_Pointer2val (GCPtr b i)) in v.
         pose proof (generation_sh__writable (heapgraph_generation g from)).
-        change (generation_sh (heapgraph_generation g from)) with (heapgraph_generation_sh g from) in H19.
-        rewrite <- Heqfsh in H19. unfold generation_data_at_.
+        change
+          (generation_sh (heapgraph_generation g from))
+          with (heapgraph_generation_sh g from)
+          in H19.
+        rewrite <- Heqfsh in H19.
+        unfold generation_data_at_.
         sep_apply (single_outlier_rep_memory_block_FF (GCPtr b i) fp gn fsh H19 v).
         assert_PROP False by entailer!. contradiction.
       * forward_if. 1: exfalso; apply H19'; reflexivity.
@@ -201,1214 +275,1549 @@ Proof.
         -- split3; [| |split3]; simpl; try rewrite <- Heqroot;
              [easy.. | constructor | hnf; intuition | apply tir_id].
         -- unfold thread_info_rep. entailer!.
-    + specialize (H14 _ H13). destruct (heapgraph_block_ptr g a) eqn:Ea ; try contradiction.
-      forward_if. 2: exfalso; apply Int.one_not_zero in H20; assumption.
-      clear H20 H20'. simpl in H15, H17. forward_call (Vptr b i).
-      rewrite <- Ea in *.
-      gather_SEP (graph_rep _) (heap_rest_rep _) (outlier_rep _).
-      rewrite <- HeqP.
-      replace_SEP 0 ((weak_derives P (memory_block fsh fn fp * TT) && emp) * P) by
-          (entailer; assumption). clear H19. Intros. assert (heapgraph_has_block g a). {
-        destruct H5. red in H19. rewrite Forall_forall in H19. apply H19.
-        rewrite <- filter_sum_right_In_iff. assumption. }
-      assert (P |-- (weak_derives P (valid_pointer (Vptr b i) * TT) && emp) * P). {
-        apply weak_derives_strong. subst. sep_apply (graph_rep_vertex_rep g a H19).
-        Intros shh. unfold vertex_rep, vertex_at. remember (heapgraph_block_cells_vals g a).
-        sep_apply (data_at_valid_ptr shh (tarray int_or_ptr_type (Zlength l)) l (heapgraph_block_ptr g a)).
-        - apply readable_nonidentity, writable_readable_share. assumption.
-        - subst l. simpl. rewrite fields_eq_length.
-          rewrite Z.max_r; pose proof (block_fields__range (heapgraph_block g a)); lia.
-        - rewrite Ea. cancel.
-      }
-      replace_SEP 1 (weak_derives P (valid_pointer (Vptr b i) * TT) && emp * P)
-        by (entailer; assumption). clear H20. Intros. rewrite <- Ea in *.
-      forward_call (fsh, fp, fn, (heapgraph_block_ptr g a), P).
+    }
+    specialize (H14 _ H13). destruct (heapgraph_block_ptr g a) eqn:Ea ; try contradiction.
+    forward_if. 2: exfalso; apply Int.one_not_zero in H20; assumption.
+    clear H20 H20'. simpl in H15, H17. forward_call (Vptr b i).
+    rewrite <- Ea in *.
+    gather_SEP (graph_rep _) (heap_rest_rep _) (outlier_rep _).
+    rewrite <- HeqP.
+    replace_SEP 0 ((weak_derives P (memory_block fsh fn fp * TT) && emp) * P) by
+        (entailer; assumption). clear H19. Intros. assert (heapgraph_has_block g a). {
+      destruct H5. red in H19. rewrite Forall_forall in H19. apply H19.
+      rewrite <- filter_sum_right_In_iff. assumption. }
+    assert (P |-- (weak_derives P (valid_pointer (Vptr b i) * TT) && emp) * P). {
+      apply weak_derives_strong. subst. sep_apply (graph_rep_vertex_rep g a H19).
+      Intros shh. unfold vertex_rep, vertex_at. remember (heapgraph_block_cells_vals g a).
+      sep_apply (data_at_valid_ptr shh (tarray int_or_ptr_type (Zlength l)) l (heapgraph_block_ptr g a)).
+      - apply readable_nonidentity, writable_readable_share. assumption.
+      - subst l. simpl. rewrite fields_eq_length.
+        rewrite Z.max_r; pose proof (block_fields__range (heapgraph_block g a)); lia.
+      - rewrite Ea. cancel.
+    }
+    replace_SEP 1 (weak_derives P (valid_pointer (Vptr b i) * TT) && emp * P)
+      by (entailer; assumption).
+    clear H20.
+    Intros.
+    rewrite <- Ea in *.
+    forward_call (fsh, fp, fn, (heapgraph_block_ptr g a), P).
+    Intros vv.
+    rewrite HeqP.
+    sep_apply (graph_and_heap_rest_v_in_range_iff _ _ _ _ H H7 H19).
+    Intros.
+    rewrite <- Heqfp, <- Heqgn, <- Heqfn in H20.
+    destruct vv.
+    2: {
+      forward_if.
       {
-        admit.
+        exfalso.
+        now apply H21'.
       }
-      Intros vv. rewrite HeqP.
-      sep_apply (graph_and_heap_rest_v_in_range_iff _ _ _ _ H H7 H19). Intros.
-      rewrite <- Heqfp, <- Heqgn, <- Heqfn in H20. destruct vv.
-      * Intros. rewrite H20 in v. clear H20. forward_if.
-        2: exfalso; inversion H20. freeze [1; 2; 3; 4; 5; 6] FR.
-        clear H20 H20'. localize [vertex_rep (heapgraph_generation_sh g (addr_gen a)) g a].
-        unfold vertex_rep, vertex_at. Intros. rewrite v.
-        assert (readable_share (heapgraph_generation_sh g from)) by
-            (unfold heapgraph_generation_sh; apply writable_readable, generation_sh__writable).
-        sep_apply (data_at_minus1_address (heapgraph_generation_sh g from) (Z2val (heapgraph_block_header g a))
-                                          (heapgraph_block_ptr g a)).
-        Intros. forward. clear H21.
-        gather_SEP (data_at _ (if Archi.ptr64 then tulong else tuint) _ _)
-                   (data_at _ _ _ _).
-        replace_SEP 0 (vertex_rep (heapgraph_generation_sh g (addr_gen a)) g a) by
-            (unfold vertex_rep, vertex_at; entailer!).
-        unlocalize [graph_rep g]. 1: apply (graph_vertex_ramif_stable _ _ H19).
-        forward_if.
-        -- try apply Int64.same_if_eq in H21.
-           pose proof (heapgraph_block_header__repr_iff g a). simpl in H22.
-           rewrite H22 in H21. clear H22.
-           localize [vertex_rep (heapgraph_generation_sh g (addr_gen a)) g a].
-           rewrite v. unfold vertex_rep, vertex_at. Intros.
-           unfold heapgraph_block_cells_vals at 2. rewrite H21.
-           assert (0 <= 0 < Zlength (heapgraph_block_cells_vals g a)). {
-             split. 1: lia. rewrite fields_eq_length.
-             apply (proj1 (block_fields__range (heapgraph_block g a))). }
-           assert (is_pointer_or_integer
-                     (heapgraph_block_ptr g (block_copied_vertex (heapgraph_block g a)))). {
-             apply isptr_is_pointer_or_integer. unfold heapgraph_block_ptr.
-             rewrite isptr_offset_val.
-             apply heapgraph_generation_base__isptr, H9; assumption. }
-           forward.
-           rewrite Znth_0_cons.
-           gather_SEP (data_at _ _ _ _)
-                      (data_at _ _ _ _).
-           replace_SEP 0 (vertex_rep (heapgraph_generation_sh g (addr_gen a)) g a). {
-             unfold vertex_rep, vertex_at. unfold heapgraph_block_cells_vals at 3.
-             rewrite H21. entailer!. }
-           unlocalize [graph_rep g]. 1: apply (graph_vertex_ramif_stable _ _ H19).
-           thaw FR. forward.
-           Exists g (upd_thread_info_arg
-                       t_info
-                       (Znth z (live_roots_indices f_info))
-                       (heapgraph_block_ptr g (block_copied_vertex (heapgraph_block g a))) H16)
-                  (upd_bunch z f_info roots (inr (block_copied_vertex (heapgraph_block g a)))).
-           unfold thread_info_rep. entailer!. 2: simpl; entailer!. simpl.
-           split; split; [|split; [|split] | |split]; auto.
-           ++ now apply upd_fun_thread_arg_compatible.
-           ++ specialize (H9 _ H19 H21). destruct H9 as [? _].
-              now apply upd_roots_compatible.
-           ++ rewrite <- Heqroot, H21.
-              now rewrite if_true by reflexivity.
-           ++ rewrite <- Heqroot. apply fr_v_in_forwarded; [reflexivity | assumption].
-           ++ easy.
-        -- forward. thaw FR. freeze [0; 1; 2; 3; 4; 5] FR.
-           try apply Int64_eq_false in H21.
-           pose proof (heapgraph_block_header__repr_iff g a). simpl in H22.
-           rewrite H22 in H21. clear H22. apply not_true_is_false in H21.
-           rewrite heapgraph_block_header__Wosize by assumption.
-           assert (0 <= Z.of_nat to < 12). {
-             clear -H H8. destruct H as [_ [_ ?]]. red in H8.
-             pose proof (heap_spaces__size (ti_heap t_info)).
-             rewrite Zlength_correct in H0. rep_lia. } unfold heap_struct_rep.
-           destruct (gt_gs_compatible _ _ H _ H8) as [H23 H24 H25 HH26].
-           simpl in H23, H24, H25, HH26.
-           rewrite nth_space_Znth in *.
-           remember (Znth (Z.of_nat to) (heap_spaces (ti_heap t_info))) as sp_to.
-           assert (isptr (space_base sp_to)) by (rewrite <- H23; apply generation_base__isptr).
-           remember (map space_tri (heap_spaces (ti_heap t_info))) as l.
-           assert (@Znth (val * (val * (val * val))) (Vundef, (Vundef, (Vundef, Vundef)))
-                         (Z.of_nat to) l = space_tri sp_to). {
-             subst l sp_to. rewrite Znth_map by (rewrite heap_spaces__size; rep_lia).
-             reflexivity. }
-           forward; rewrite H27; unfold space_tri. 1: entailer!.
-           forward. simpl sem_binary_operation'.
-           rewrite sapi_ptr_val; [|assumption | rep_lia].
-           Opaque Znth. forward. Transparent Znth.
-           rewrite sapil_ptr_val by assumption. rewrite H27. unfold space_tri.
-           rewrite <- Z.add_assoc.
-           replace (1 + Zlength (block_fields (heapgraph_block g a))) with (heapgraph_block_size g a) by
-               (unfold heapgraph_block_size; lia). thaw FR. freeze [0; 2; 3; 4; 5; 6] FR.
-           assert (Hi : 0 <= Z.of_nat to < Zlength (heap_spaces (ti_heap t_info))) by
-               (rewrite heap_spaces__size; rep_lia).
-           assert (Hh: has_space (Znth (Z.of_nat to) (heap_spaces (ti_heap t_info)))
-                                 (heapgraph_block_size g a)). {
-             red. split. 1: pose proof (heapgraph_block_size__one g a); lia.
-             transitivity (unmarked_gen_size g (addr_gen a)).
-             - apply single_unmarked_le; assumption.
-             - red in H1. unfold rest_gen_size in H1. subst from.
-               rewrite nth_space_Znth in H1.
-               lia.
-           }
-           assert (Hn: space_base (Znth (Z.of_nat to) (heap_spaces (ti_heap t_info))) <>
-                       nullval). {
-             rewrite <- Heqsp_to. destruct (space_base sp_to); try contradiction.
-             intro Hn. inversion Hn. }
-           rewrite (heap_rest_rep_cut
-                      (ti_heap t_info) (Z.of_nat to) (heapgraph_block_size g a) Hi Hh Hn).
-           rewrite <- Heqsp_to. thaw FR.
-           gather_SEP (data_at _ thread_info_type _ _)
-                      (data_at _ heap_type _ _)
-                      (heap_rest_rep _).
-           replace_SEP 0 (thread_info_rep
-                            sh (cut_thread_info t_info _ _ Hi Hh) ti). {
-             entailer. unfold thread_info_rep. simpl ti_heap. simpl ti_heap_p. cancel.
-             simpl heap_spaces. rewrite <- upd_Znth_map. unfold cut_space.
-             unfold space_tri at 3. simpl. unfold heap_struct_rep. cancel. }
-           sep_apply (graph_vertex_ramif_stable _ _ H19). Intros.
-           freeze [1; 2; 3; 4; 5] FR. rewrite v.
-           remember (heapgraph_generation_sh g from) as shv.
-           assert (writable_share (space_sh sp_to)) by
-               (rewrite <- H24; apply generation_sh__writable).
-           remember (space_sh sp_to) as sht.
-           rewrite (data_at__tarray_value _ _ 1). 2: unfold heapgraph_block_size; rep_lia.
-           Intros.
-           remember (offset_val (WORD_SIZE * space_allocated sp_to) (space_base sp_to)).
-           rewrite (data_at__int_or_ptr_integer sht v0).
-           assert_PROP
-             (force_val (sem_add_ptr_int
-                           (if Archi.ptr64 then tulong else tuint) Signed
-                           (offset_val (WORD_SIZE * (space_allocated sp_to + 1))
-                                       (space_base sp_to))
-                           (eval_unop Oneg tint (vint 1))) =
-              field_address (if Archi.ptr64 then tulong else tuint) [] v0). {
-             subst v0. entailer!. simpl. rewrite neg_repr.
-             rewrite sem_add_pi_ptr_special; auto. 2: rep_lia. simpl in *.
-             unfold field_address. rewrite if_true by assumption.
-             simpl. rewrite !offset_offset_val. f_equal. unfold WORD_SIZE. lia. }
-           forward. sep_apply (field_at_data_at_cancel
-                                 sht (if Archi.ptr64 then tulong else tuint)
-                                 (Z2val (heapgraph_block_header g a)) v0). clear H29.
-           subst v0. rewrite offset_offset_val.
-           replace (heapgraph_block_size g a - 1) with (Zlength (block_fields (heapgraph_block g a)))
-             by (unfold heapgraph_block_size; lia).
-           replace (WORD_SIZE * space_allocated sp_to + WORD_SIZE * 1) with
-               (WORD_SIZE * (space_allocated sp_to + 1))%Z by rep_lia.
-           remember (offset_val (WORD_SIZE * (space_allocated sp_to + 1))
-                                (space_base sp_to)) as nv.
-           thaw FR. freeze [0; 1; 2; 3; 4; 5] FR. rename i into j.
-           remember (Zlength (block_fields (heapgraph_block g a))) as n.
-           assert (isptr nv) by (subst nv; rewrite isptr_offset_val; assumption).
-           remember (field_address thread_info_type
-                                   [ArraySubsc (Znth z (live_roots_indices f_info));
-                                    StructField _args] ti) as p_addr.
-           remember (field_address heap_type
-                                   [StructField _next; ArraySubsc (Z.of_nat to);
-                                    StructField _spaces] (ti_heap_p t_info)) as n_addr.
-           forward_for_simple_bound
-             n
-             (EX i: Z,
-              PROP ( )
-              LOCAL (temp _new nv;
-                     temp _sz (if Archi.ptr64 then Vlong (Int64.repr n) else vint n);
-                     temp _v (heapgraph_block_ptr g a);
-                     temp _from_start fp;
-                     temp _from_limit (offset_val fn fp);
-                     temp _next n_addr;
-                     temp _p p_addr;
-                     temp _depth (vint depth))
-              SEP (vertex_rep shv g a;
-                   data_at sht (tarray int_or_ptr_type i)
-                           (sublist 0 i (heapgraph_block_cells_vals g a)) nv;
-                   data_at_ sht (tarray int_or_ptr_type (n - i))
-                            (offset_val (WORD_SIZE * i) nv); FRZL FR))%assert.
-           ++ pose proof (block_fields__range2 (heapgraph_block g a)). simpl in H30.
-              now rewrite <- Heqn in H30.
-           ++ rewrite sublist_nil. replace (n - 0) with n by lia.
-              replace (WORD_SIZE * 0)%Z with 0 by lia.
-              rewrite isptr_offset_val_zero by assumption.
-              rewrite data_at_zero_array_eq;
-                [|reflexivity | assumption | reflexivity]. entailer!.
-              admit.
-           ++ unfold vertex_rep, vertex_at. Intros.
-              rewrite fields_eq_length, <- Heqn. forward.
-              ** entailer!. pose proof (mfv_all_is_ptr_or_int _ _ H9 H10 H19).
-                 rewrite Forall_forall in H45.
-                 apply H45, Znth_In.
-                 now rewrite fields_eq_length.
-              ** rewrite (data_at__tarray_value _ _ 1) by lia. Intros.
-                 rewrite data_at__singleton_array_eq.
-                 assert_PROP
-                   (field_compatible int_or_ptr_type []
-                                     (offset_val (WORD_SIZE * i) nv)) by
-                     (sep_apply (data_at__local_facts
-                                   sht int_or_ptr_type
-                                   (offset_val (WORD_SIZE * i) nv)); entailer!).
-                 assert_PROP
-                   ((if Archi.ptr64 then
-                      force_val (sem_add_ptr_long int_or_ptr_type
-                                                  nv (Vlong (Int64.repr i)))
-                     else force_val (sem_add_ptr_int int_or_ptr_type
-                                                     Signed nv (vint i)))=
-                    field_address int_or_ptr_type []
-                                  (offset_val (WORD_SIZE * i) nv)). {
-                   unfold field_address. rewrite if_true by assumption.
-                   clear. entailer!. } simpl in H32.
-                 gather_SEP (data_at _ _ _
-                                     (offset_val (- WORD_SIZE) (heapgraph_block_ptr g a)))
-                            (data_at _ _ _ (heapgraph_block_ptr g a)).
-                 replace_SEP 0 (vertex_rep shv g a) by
-                     (unfold vertex_rep, vertex_at;
-                      rewrite fields_eq_length; entailer!). forward.
-                 rewrite offset_offset_val.
-                 replace (n - i - 1) with (n - (i + 1)) by lia.
-                 replace (WORD_SIZE * i + WORD_SIZE * 1) with
-                     (WORD_SIZE * (i + 1))%Z by lia.
-                 gather_SEP (data_at sht _ _ nv) (field_at _ _ _ _ _).
-                 rewrite data_at_mfs_eq. 2: assumption.
-                 2: subst n; assumption. entailer!.
-           ++ thaw FR. rewrite v, <- Heqshv.
-              gather_SEP (vertex_rep _ _ _) (_ -* _).
-              replace_SEP 0 (graph_rep g) by (entailer!; apply wand_frame_elim).
-              rewrite sublist_all by (rewrite fields_eq_length; lia).
-              replace_SEP 2 emp. {
-                replace (n - n) with 0 by lia. clear. entailer.
-                apply data_at__value_0_size. }
-              assert (nv = heapgraph_block_ptr g (new_copied_v g to)). {
-                subst nv. unfold heapgraph_block_ptr. unfold new_copied_v. simpl. f_equal.
-                - unfold heapgraph_block_offset. simpl. rewrite H25. reflexivity.
-                - unfold heapgraph_generation_base. rewrite if_true by assumption.
-                  rewrite H23. reflexivity. }
-              gather_SEP (data_at _ _ _ nv) (emp)
-              (data_at sht (if Archi.ptr64 then tulong else tuint) _ _).
-              replace_SEP
-                0 (vertex_at (heapgraph_generation_sh g to)
-                             (heapgraph_block_ptr g (new_copied_v g to))
-                             (heapgraph_block_header g a) (heapgraph_block_cells_vals g a)). {
-                normalize. rewrite <- H24.
-                change (generation_sh (heapgraph_generation g to)) with (heapgraph_generation_sh g to).
-                rewrite <- fields_eq_length in Heqn.
-                replace (offset_val (WORD_SIZE * space_allocated sp_to) (space_base sp_to))
-                  with (offset_val (- WORD_SIZE) nv) by
-                    (rewrite Heqnv; rewrite offset_offset_val; f_equal; rep_lia).
-                rewrite <- H30. unfold vertex_at; entailer!. }
-              gather_SEP (vertex_at _ _ _ _) (graph_rep _).
-              rewrite (copied_v_derives_new_g g a to) by assumption.
-              freeze [1; 2; 3; 4] FR. remember (lgraph_add_copied_v g a to) as g'.
-              assert (heapgraph_block_ptr g' a = heapgraph_block_ptr g a) by
-                  (subst g'; apply lacv_heapgraph_block_ptr_old; assumption).
-              assert (heapgraph_block_ptr g' (new_copied_v g to) =
-                      heapgraph_block_ptr g (new_copied_v g to)) by
-                  (subst g'; apply lacv_heapgraph_block_ptr_new; assumption).
-              rewrite <- H31. rewrite <- H32 in H30.
-              assert (writable_share (heapgraph_generation_sh g' (addr_gen a))) by
-                  (unfold heapgraph_generation_sh; apply generation_sh__writable).
-              assert (heapgraph_has_block g' (new_copied_v g to)) by
-                  (subst g'; apply lacv_heapgraph_has_block_new; assumption).
-              sep_apply (graph_rep_valid_int_or_ptr _ _ H34). Intros.
-              rewrite <- H30 in H35. assert (heapgraph_has_block g' a) by
-                  (subst g'; apply lgraph_add_copied_v__heapgraph_has_block; assumption).
-              remember (heapgraph_generation_sh g' (addr_gen a)) as sh'.
-              sep_apply (graph_vertex_lmc_ramif g' a (new_copied_v g to) H36).
-              rewrite <- Heqsh'. Intros. freeze [1; 2] FR1.
-              unfold vertex_rep, vertex_at. Intros.
-              sep_apply (data_at_minus1_address
-                           sh' (Z2val (heapgraph_block_header g' a)) (heapgraph_block_ptr g' a)).
-              Intros. forward. clear H37. try rewrite Int.signed_repr by rep_lia.
-              sep_apply (field_at_data_at_cancel
-                           sh' (if Archi.ptr64 then tulong else tuint)
-                           (if Archi.ptr64 then (Vlong (Int64.repr 0)) else (vint 0))
-                           (offset_val (- WORD_SIZE) (heapgraph_block_ptr g' a))).
-              forward_call (nv). remember (heapgraph_block_cells_vals g' a) as l'.
-              assert (0 < Zlength l'). {
-                subst l'. rewrite fields_eq_length.
-                apply (proj1 (block_fields__range (heapgraph_block g' a))). }
-              rewrite data_at_tarray_value_split_1 by assumption. Intros.
-              assert_PROP (force_val (sem_add_ptr_int int_or_ptr_type Signed
-                                                      (heapgraph_block_ptr g' a) (vint 0)) =
-                           field_address int_or_ptr_type [] (heapgraph_block_ptr g' a)). {
-                clear. entailer!. unfold field_address. rewrite if_true by assumption.
-                simpl. rewrite isptr_offset_val_zero. 1: reflexivity.
-                destruct H7 ; try assumption. } forward. clear H38.
-              sep_apply (field_at_data_at_cancel
-                           sh' int_or_ptr_type nv (heapgraph_block_ptr g' a)).
-              gather_SEP
-                (data_at _ (if Archi.ptr64 then tulong else tuint) _ _)
-                (data_at _ int_or_ptr_type nv _)
-                (data_at _ _ _ _).
-              rewrite H30. subst l'.
-              rewrite <- lmc_vertex_rep_eq.
-              thaw FR1.
-              gather_SEP (vertex_rep _ _ _) (_ -* _).
-              sep_apply
-                (wand_frame_elim
-                   (vertex_rep sh' (lgraph_mark_copied g' a (new_copied_v g to)) a)
-                   (graph_rep (lgraph_mark_copied g' a (new_copied_v g to)))).
-              rewrite <- (lmc_heapgraph_block_ptr g' a (new_copied_v g to)) in *. subst g'.
-              change (lgraph_mark_copied
-                        (lgraph_add_copied_v g a to) a (new_copied_v g to))
-                with (lgraph_copy_v g a to) in *.
-              remember (lgraph_copy_v g a to) as g'. rewrite <- H30 in *. thaw FR.
-              forward_call (nv). subst p_addr.
-              remember (cut_thread_info t_info (Z.of_nat to) (heapgraph_block_size g a) Hi Hh)
-                as t_info'. unfold thread_info_rep. Intros. forward.
-              remember (Znth z (live_roots_indices f_info)) as lz.
-              gather_SEP
-                (data_at sh thread_info_type _ ti)
-                (heap_struct_rep sh _ _)
-                (heap_rest_rep _ ).
-              replace_SEP 0 (thread_info_rep
-                               sh (update_thread_info_arg t_info' lz nv H16) ti). {
-                unfold thread_info_rep. simpl heap_head. simpl ti_heap_p.
-                simpl ti_args. simpl ti_heap. clear Heqt_info'. entailer!. }
-              remember (update_thread_info_arg t_info' lz nv H16) as t. subst t_info'.
-              rename t into t_info'. rewrite H30 in H32.
-              assert (forward_relation from to 0 (inl (inr a)) g g') by
-                  (subst g'; constructor; assumption).
-              assert (forward_condition g' t_info' from to). {
-                subst g' t_info' from. apply lcv_forward_condition; try assumption.
-                red. intuition. }
-              remember (upd_bunch z f_info roots (inr (new_copied_v g to))) as roots'.
-              assert (super_compatible (g', t_info', roots') f_info outlier). {
-                subst g' t_info' roots' lz. rewrite H30, H32.
-                apply lcv_super_compatible; try assumption. red. intuition. }
-              assert (thread_info_relation t_info t_info'). {
-                subst t_info'. split; [|split]; [reflexivity| |]; intros m.
-                - rewrite utiacti_gen_size. reflexivity.
-                - rewrite utiacti_space_base. reflexivity. }
-              forward_if.
-              ** destruct H41 as [? [? ?]]. replace fp with (heapgraph_generation_base g' from) by
-                     (subst fp g'; apply lcv_gen_start; assumption).
-                 replace (offset_val fn (heapgraph_generation_base g' from)) with
-                     (limit_address g' t_info' from) by admit.
-                     (* (subst fn gn; rewrite H43; reflexivity). *)
-                 replace n_addr with (next_address t_info' to) by
-                     (subst n_addr; rewrite H41; reflexivity).
-                 forward_for_simple_bound
-                   n
-                   (EX i: Z, EX g3: HeapGraph, EX t_info3: thread_info,
-                    PROP (super_compatible (g3, t_info3, roots') f_info outlier;
-                          forward_loop
-                            from to (Z.to_nat (depth - 1))
-                            (sublist 0 i (heapgraph_field_pairs g' (new_copied_v g to)))
-                            g' g3;
-                          forward_condition g3 t_info3 from to;
-                          thread_info_relation t_info' t_info3)
-                    LOCAL (temp _new nv;
-                           temp _sz (if Archi.ptr64 then
-                                       Vlong (Int64.repr n) else vint n);
-                           temp _from_start (heapgraph_generation_base g3 from);
-                           temp _from_limit (limit_address g3 t_info3 from);
-                           temp _next (next_address t_info3 to);
-                           temp _depth (vint depth))
-                    SEP (all_string_constants rsh gv;
-                         fun_info_rep rsh f_info fi;
-                         outlier_rep outlier;
-                         graph_rep g3;
-                         thread_info_rep sh t_info3 ti))%assert.
-                 --- pose proof (block_fields__range2 (heapgraph_block g a)). simpl in H45.
-                     now rewrite <- Heqn in H45.
-                 --- Exists g' t_info'. autorewrite with sublist.
-                     assert (forward_loop from to (Z.to_nat (depth - 1)) [] g' g') by
-                         constructor. unfold thread_info_relation. entailer!.
-                 --- change (Tpointer tvoid {| attr_volatile := false;
-                                               attr_alignas := Some 2%N |})
-                       with (int_or_ptr_type). Intros.
-                     assert (heapgraph_has_gen g' to) by
-                         (rewrite Heqg', <- lcv_graph_has_gen; assumption).
-                     assert (heapgraph_has_block g' (new_copied_v g to)) by
-                         (rewrite Heqg'; apply lcv_heapgraph_has_block_new; assumption).
-                     forward_call (rsh, sh, gv, fi, ti, g3, t_info3, f_info, roots',
-                                   outlier, from, to, depth - 1,
-                                   (@inr Z _ (new_copied_v g to, i))).
-                     +++ apply prop_right. simpl. rewrite sub_repr, H30.
-                         do 4 f_equal.
-                         first [rewrite sem_add_pi_ptr_special' |
-                                rewrite sem_add_pl_ptr_special']; auto.
-                         *** simpl. f_equal. erewrite fl_heapgraph_block_ptr; eauto.
-                             subst g'. apply heapgraph_has_block_in_closure. assumption.
-                         *** rewrite <- H30. assumption.
-                     +++ split3; [| |split].
-                         *** apply (fl_heapgraph_has_block _ _ _ _ _ _ H50 H47 _ H51).
-                         *** erewrite <- fl_block_fields; eauto. subst g'.
-                             unfold lgraph_copy_v. subst n.
-                             rewrite <- lmc_block_fields, lacv_vlabel_new.
-                             assumption.
-                         *** erewrite <- fl_block_mark; eauto. subst g' from.
-                             rewrite lcv_vlabel_new. auto. assumption.
-                         *** simpl. lia.
-                     +++ Intros vret. destruct vret as [[g4 t_info4] roots4].
-                         simpl fst in *. simpl snd in *. Exists g4 t_info4.
-                         simpl in H53. subst roots4.
-                         assert (heapgraph_generation_base g3 from = heapgraph_generation_base g4 from). {
-                           eapply fr_gen_start; eauto.
-                           erewrite <- fl_graph_has_gen; eauto. } rewrite H53.
-                         assert (limit_address g3 t_info3 from =
-                                 limit_address g4 t_info4 from). {
-                           unfold limit_address. f_equal. 2: assumption. f_equal.
-                           rewrite (thread_info_relation__space_remembered _ _ _ H56).
-                           destruct H56 as [? [? _]].
-                           rewrite H57.
-                           reflexivity.
-                         }
-                         rewrite H57.
-                         assert (next_address t_info3 to = next_address t_info4 to). {
-                           unfold next_address. f_equal. destruct H56. assumption. }
-                         rewrite H58. clear H53 H57 H58.
-                         assert (thread_info_relation t_info' t_info4) by
-                             (apply tir_trans with t_info3; assumption).
-                         assert (forward_loop
-                                   from to (Z.to_nat (depth - 1))
-                                   (sublist 0 (i + 1)
-                                            (heapgraph_field_pairs g' (new_copied_v g to)))
-                                   g' g4). {
-                           eapply forward_loop_add_tail_vpp; eauto. subst n g' from.
-                           rewrite lcv_vlabel_new; assumption. }
-                         entailer!.
-                 --- Intros g3 t_info3.
-                     assert (thread_info_relation t_info t_info3) by
-                         (apply tir_trans with t_info';
-                          [split; [|split]|]; assumption).
-                     rewrite sublist_all in H46. clear Heqt.
-                     2: { rewrite Z.le_lteq. right. subst n g' from.
-                          rewrite heapgraph_field_pairs__Zlength, lcv_vlabel_new; auto. }
-                     Opaque super_compatible.
-                     Exists g3 t_info3 roots'. entailer!. simpl.
-                     rewrite <- Heqroot, H21, if_true by reflexivity. split; auto.
-                     replace (Z.to_nat depth) with (S (Z.to_nat (depth - 1))) by
-                         (rewrite <- Z2Nat.inj_succ; [f_equal|]; lia).
-                     constructor; easy.
-                     Transparent super_compatible.
-              ** assert (depth = 0) by lia. subst depth. clear H42.
-                 clear Heqnv. forward.
-                 remember (cut_thread_info
-                             t_info (Z.of_nat to) (heapgraph_block_size g a) Hi Hh).
-                 Exists (lgraph_copy_v g a to) (update_thread_info_arg t lz nv H16)
-                        (upd_bunch z f_info roots (inr (new_copied_v g to))).
-                 entailer!. simpl; rewrite <- Heqroot.
-                 rewrite if_true by reflexivity; rewrite H21; easy.
-      * forward_if. 1: exfalso; apply H21'; reflexivity.
-        rewrite H20 in n. forward.
-        Exists g t_info roots. entailer!; simpl.
-        -- rewrite <- Heqroot, if_false by assumption.
-           split3; [| |simpl root2forward; constructor]; try easy.
-           now constructor.
-        -- unfold thread_info_rep. entailer!.
+      rewrite H20 in n.
+      forward.
+      Exists g t_info roots.
+      entailer! ; simpl.
+      - rewrite <- Heqroot, if_false by assumption.
+        split3; [| |simpl root2forward; constructor]; try easy.
+        now constructor.
+      - unfold thread_info_rep. entailer!.
+    }
+    Intros.
+    rewrite H20 in v.
+    clear H20.
+    forward_if.
+    2: {
+      exfalso.
+      now inversion H20.
+    }
+    freeze [1; 2; 3; 4; 5; 6] FR.
+    clear H20 H20'.
+    localize [vertex_rep (heapgraph_generation_sh g (addr_gen a)) g a].
+    unfold vertex_rep, vertex_at.
+    Intros.
+    rewrite v.
+    assert
+      (readable_share (heapgraph_generation_sh g from))
+      as H20
+      by (unfold heapgraph_generation_sh; apply writable_readable, generation_sh__writable).
+    sep_apply (
+      data_at_minus1_address
+        (heapgraph_generation_sh g from)
+        (Z2val (heapgraph_block_header g a))
+        (heapgraph_block_ptr g a)
+    ).
+    Intros.
+    forward.
+    clear H21.
+    gather_SEP (data_at _ (if Archi.ptr64 then tulong else tuint) _ _) (data_at _ _ _ _).
+    replace_SEP 0
+      (vertex_rep (heapgraph_generation_sh g (addr_gen a)) g a)
+      by (unfold vertex_rep, vertex_at; entailer!).
+    unlocalize [graph_rep g].
+    {
+      apply (graph_vertex_ramif_stable _ _ H19).
+    }
+    forward_if.
+    {
+      try apply Int64.same_if_eq in H21.
+      pose proof (heapgraph_block_header__repr_iff g a).
+      simpl in H22.
+      rewrite H22 in H21.
+      clear H22.
+      localize [vertex_rep (heapgraph_generation_sh g (addr_gen a)) g a].
+      rewrite v.
+      unfold vertex_rep, vertex_at.
+      Intros.
+      unfold heapgraph_block_cells_vals at 2.
+      rewrite H21.
+      assert
+        (0 <= 0 < Zlength (heapgraph_block_cells_vals g a))
+        as H22.
+      {
+        split. 1: lia. rewrite fields_eq_length.
+        apply (proj1 (block_fields__range (heapgraph_block g a))).
+      }
+      assert
+        (is_pointer_or_integer (heapgraph_block_ptr g (block_copied_vertex (heapgraph_block g a))))
+        as H23.
+      {
+        apply isptr_is_pointer_or_integer. unfold heapgraph_block_ptr.
+        rewrite isptr_offset_val.
+        apply heapgraph_generation_base__isptr, H9; assumption.
+      }
+      forward.
+      rewrite Znth_0_cons.
+      gather_SEP (data_at _ _ _ _) (data_at _ _ _ _).
+      replace_SEP 0
+        (vertex_rep (heapgraph_generation_sh g (addr_gen a)) g a).
+      {
+        unfold vertex_rep, vertex_at.
+        unfold heapgraph_block_cells_vals at 3.
+        rewrite H21.
+        entailer!.
+      }
+      unlocalize [graph_rep g].
+      {
+        apply (graph_vertex_ramif_stable _ _ H19).
+      }
+      thaw FR.
+      forward.
+      Exists g (upd_thread_info_arg
+                  t_info
+                  (Znth z (live_roots_indices f_info))
+                  (heapgraph_block_ptr g (block_copied_vertex (heapgraph_block g a))) H16)
+            (upd_bunch z f_info roots (inr (block_copied_vertex (heapgraph_block g a)))).
+      unfold thread_info_rep.
+      entailer!.
+      2: {
+        simpl.
+        entailer!.
+      }
+      simpl.
+      split; split; [|split; [|split] | |split] ; try easy.
+      - now apply upd_fun_thread_arg_compatible.
+      - specialize (H9 _ H19 H21). destruct H9 as [? _].
+        now apply upd_roots_compatible.
+      - rewrite <- Heqroot, H21.
+        now rewrite if_true by reflexivity.
+      - rewrite <- Heqroot.
+        now apply fr_v_in_forwarded.
+    }
+    forward.
+    thaw FR.
+    freeze [0; 1; 2; 3; 4; 5] FR.
+    try apply Int64_eq_false in H21.
+    pose proof (heapgraph_block_header__repr_iff g a). simpl in H22.
+    rewrite H22 in H21. clear H22. apply not_true_is_false in H21.
+    rewrite heapgraph_block_header__Wosize by assumption.
+    assert (0 <= Z.of_nat to < 12). {
+      clear -H H8. destruct H as [_ [_ ?]]. red in H8.
+      pose proof (heap_spaces__size (ti_heap t_info)).
+      rewrite Zlength_correct in H0. rep_lia. } unfold heap_struct_rep.
+    destruct (gt_gs_compatible _ _ H _ H8) as [H23 H24 H25 HH26].
+    simpl in H23, H24, H25, HH26.
+    rewrite nth_space_Znth in *.
+    remember (Znth (Z.of_nat to) (heap_spaces (ti_heap t_info))) as sp_to.
+    assert (isptr (space_base sp_to)) by (rewrite <- H23; apply generation_base__isptr).
+    remember (map space_tri (heap_spaces (ti_heap t_info))) as l.
+    assert (@Znth (val * (val * (val * val))) (Vundef, (Vundef, (Vundef, Vundef)))
+                  (Z.of_nat to) l = space_tri sp_to). {
+      subst l sp_to. rewrite Znth_map by (rewrite heap_spaces__size; rep_lia).
+      reflexivity. }
+    forward; rewrite H27; unfold space_tri. 1: entailer!.
+    forward. simpl sem_binary_operation'.
+    rewrite sapi_ptr_val; [|assumption | rep_lia].
+    Opaque Znth. forward. Transparent Znth.
+    rewrite sapil_ptr_val by assumption. rewrite H27. unfold space_tri.
+    rewrite <- Z.add_assoc.
+    replace (1 + Zlength (block_fields (heapgraph_block g a))) with (heapgraph_block_size g a) by
+        (unfold heapgraph_block_size; lia). thaw FR. freeze [0; 2; 3; 4; 5; 6] FR.
+    assert (Hi : 0 <= Z.of_nat to < Zlength (heap_spaces (ti_heap t_info))) by
+        (rewrite heap_spaces__size; rep_lia).
+    assert (Hh: has_space (Znth (Z.of_nat to) (heap_spaces (ti_heap t_info)))
+                          (heapgraph_block_size g a)). {
+      red. split. 1: pose proof (heapgraph_block_size__one g a); lia.
+      transitivity (unmarked_gen_size g (addr_gen a)).
+      - apply single_unmarked_le; assumption.
+      - red in H1. unfold rest_gen_size in H1. subst from.
+        rewrite nth_space_Znth in H1.
+        lia.
+    }
+    assert (Hn: space_base (Znth (Z.of_nat to) (heap_spaces (ti_heap t_info))) <>
+                nullval). {
+      rewrite <- Heqsp_to. destruct (space_base sp_to); try contradiction.
+      intro Hn. inversion Hn. }
+    rewrite (heap_rest_rep_cut
+              (ti_heap t_info) (Z.of_nat to) (heapgraph_block_size g a) Hi Hh Hn).
+    rewrite <- Heqsp_to. thaw FR.
+    gather_SEP (data_at _ thread_info_type _ _)
+              (data_at _ heap_type _ _)
+              (heap_rest_rep _).
+    replace_SEP 0 (thread_info_rep
+                    sh (cut_thread_info t_info _ _ Hi Hh) ti). {
+      entailer. unfold thread_info_rep. simpl ti_heap. simpl ti_heap_p. cancel.
+      simpl heap_spaces. rewrite <- upd_Znth_map. unfold cut_space.
+      unfold space_tri at 3. simpl. unfold heap_struct_rep. cancel. }
+    sep_apply (graph_vertex_ramif_stable _ _ H19).
+    Intros.
+    freeze [1; 2; 3; 4; 5] FR.
+    rewrite v.
+    remember (heapgraph_generation_sh g from) as shv.
+    assert
+      (writable_share (space_sh sp_to))
+      as H28
+      by (rewrite <- H24; apply generation_sh__writable).
+    remember (space_sh sp_to) as sht.
+    rewrite (data_at__tarray_value _ _ 1).
+    2: {
+      unfold heapgraph_block_size.
+      rep_lia.
+    }
+    Intros.
+    remember (offset_val (WORD_SIZE * space_allocated sp_to) (space_base sp_to)).
+    rewrite (data_at__int_or_ptr_integer sht v0).
+    assert_PROP (
+      force_val (sem_add_ptr_int
+                  (if Archi.ptr64 then tulong else tuint) Signed
+                  (offset_val (WORD_SIZE * (space_allocated sp_to + 1)) (space_base sp_to))
+                  (eval_unop Oneg tint (vint 1)))
+      = field_address (if Archi.ptr64 then tulong else tuint) [] v0)
+      as H29.
+    {
+      subst v0. entailer!. simpl. rewrite neg_repr.
+      rewrite sem_add_pi_ptr_special; auto. 2: rep_lia. simpl in *.
+      unfold field_address. rewrite if_true by assumption.
+      simpl. rewrite !offset_offset_val. f_equal. unfold WORD_SIZE. lia.
+    }
+    forward.
+    sep_apply (field_at_data_at_cancel sht (if Archi.ptr64 then tulong else tuint) (Z2val (heapgraph_block_header g a)) v0).
+    clear H29.
+    subst v0.
+    rewrite offset_offset_val.
+    replace
+      (heapgraph_block_size g a - 1)
+      with (Zlength (block_fields (heapgraph_block g a)))
+      by (unfold heapgraph_block_size; lia).
+    replace
+      (WORD_SIZE * space_allocated sp_to + WORD_SIZE * 1)
+      with (WORD_SIZE * (space_allocated sp_to + 1))%Z
+      by rep_lia.
+    remember (offset_val (WORD_SIZE * (space_allocated sp_to + 1)) (space_base sp_to)) as nv eqn:Heqnv.
+    thaw FR.
+    freeze [0; 1; 2; 3; 4; 5] FR.
+    rename i into j.
+    remember
+      (Zlength (block_fields (heapgraph_block g a)))
+      as n.
+    assert
+      (isptr nv)
+      as H29
+      by (subst nv; rewrite isptr_offset_val; assumption).
+    remember
+      (field_address thread_info_type [ArraySubsc (Znth z (live_roots_indices f_info)); StructField _args] ti)
+      as p_addr eqn:Heqp_addr.
+    remember
+      (field_address heap_type [StructField _next; ArraySubsc (Z.of_nat to); StructField _spaces] (ti_heap_p t_info))
+      as n_addr eqn:Heqn_addr.
+    forward_for_simple_bound
+      n
+      (EX i: Z,
+      PROP ( )
+      LOCAL
+        ( temp _new nv
+        ; temp _sz (if Archi.ptr64 then Vlong (Int64.repr n) else vint n)
+        ; temp _v (heapgraph_block_ptr g a)
+        ; temp _from_start fp
+        ; temp _from_limit (offset_val fn fp)
+        ; temp _next n_addr
+        ; temp _p p_addr
+        ; temp _depth (vint depth)
+        )
+      SEP
+        ( vertex_rep shv g a
+        ; data_at sht (tarray int_or_ptr_type i) (sublist 0 i (heapgraph_block_cells_vals g a)) nv
+        ; data_at_ sht (tarray int_or_ptr_type (n - i)) (offset_val (WORD_SIZE * i) nv); FRZL FR
+        ))%assert.
+    {
+      pose proof (block_fields__range2 (heapgraph_block g a)) as H30.
+      simpl in H30.
+      now rewrite <- Heqn in H30.
+    }
+    {
+      rewrite sublist_nil.
+      replace (n - 0) with n by lia.
+      replace (WORD_SIZE * 0)%Z with 0 by lia.
+      rewrite isptr_offset_val_zero by assumption.
+      rewrite data_at_zero_array_eq by easy.
+      entailer!.
+    }
+    {
+      unfold vertex_rep, vertex_at. Intros.
+      rewrite fields_eq_length, <- Heqn. forward.
+      {
+        entailer!. pose proof (mfv_all_is_ptr_or_int _ _ H9 H10 H19).
+        rewrite Forall_forall in H45.
+        apply H45, Znth_In.
+        now rewrite fields_eq_length.
+      }
+      rewrite (data_at__tarray_value _ _ 1) by lia. Intros.
+      rewrite data_at__singleton_array_eq.
+      assert_PROP
+        (field_compatible int_or_ptr_type []
+                          (offset_val (WORD_SIZE * i) nv)) by
+          (sep_apply (data_at__local_facts
+                        sht int_or_ptr_type
+                        (offset_val (WORD_SIZE * i) nv)); entailer!).
+      assert_PROP
+        ((if Archi.ptr64 then
+          force_val (sem_add_ptr_long int_or_ptr_type
+                                      nv (Vlong (Int64.repr i)))
+          else force_val (sem_add_ptr_int int_or_ptr_type
+                                          Signed nv (vint i)))=
+        field_address int_or_ptr_type []
+                      (offset_val (WORD_SIZE * i) nv)). {
+        unfold field_address. rewrite if_true by assumption.
+        clear. entailer!. } simpl in H32.
+      gather_SEP (data_at _ _ _
+                          (offset_val (- WORD_SIZE) (heapgraph_block_ptr g a)))
+                (data_at _ _ _ (heapgraph_block_ptr g a)).
+      replace_SEP 0 (vertex_rep shv g a) by
+          (unfold vertex_rep, vertex_at;
+          rewrite fields_eq_length; entailer!). forward.
+      rewrite offset_offset_val.
+      replace (n - i - 1) with (n - (i + 1)) by lia.
+      replace (WORD_SIZE * i + WORD_SIZE * 1) with
+          (WORD_SIZE * (i + 1))%Z by lia.
+      gather_SEP (data_at sht _ _ nv) (field_at _ _ _ _ _).
+      rewrite data_at_mfs_eq ; subst n ; try easy.
+      entailer!.
+    }
+    thaw FR.
+    rewrite v, <- Heqshv.
+    gather_SEP (vertex_rep _ _ _) (_ -* _).
+    replace_SEP 0 (graph_rep g) by (entailer!; apply wand_frame_elim).
+    rewrite sublist_all by (rewrite fields_eq_length; lia).
+    replace_SEP 2 emp.
+    {
+      replace (n - n) with 0 by lia. clear. entailer.
+      apply data_at__value_0_size.
+    }
+    assert
+      (nv = heapgraph_block_ptr g (new_copied_v g to))
+      as H30.
+    {
+      subst nv. unfold heapgraph_block_ptr. unfold new_copied_v. simpl. f_equal.
+      - unfold heapgraph_block_offset. simpl. rewrite H25. reflexivity.
+      - unfold heapgraph_generation_base. rewrite if_true by assumption.
+        rewrite H23. reflexivity.
+    }
+    gather_SEP (data_at _ _ _ nv) (emp)
+    (data_at sht (if Archi.ptr64 then tulong else tuint) _ _).
+    replace_SEP 0 (
+      vertex_at
+        (heapgraph_generation_sh g to)
+        (heapgraph_block_ptr g (new_copied_v g to))
+        (heapgraph_block_header g a)
+        (heapgraph_block_cells_vals g a)
+    ).
+    {
+      normalize. rewrite <- H24.
+      change (generation_sh (heapgraph_generation g to)) with (heapgraph_generation_sh g to).
+      rewrite <- fields_eq_length in Heqn.
+      replace (offset_val (WORD_SIZE * space_allocated sp_to) (space_base sp_to))
+        with (offset_val (- WORD_SIZE) nv) by
+          (rewrite Heqnv; rewrite offset_offset_val; f_equal; rep_lia).
+      rewrite <- H30. unfold vertex_at; entailer!.
+    }
+    gather_SEP (vertex_at _ _ _ _) (graph_rep _).
+    rewrite (copied_v_derives_new_g g a to) by assumption.
+    freeze [1; 2; 3; 4] FR.
+    remember (lgraph_add_copied_v g a to) as g'.
+    assert
+      (heapgraph_block_ptr g' a = heapgraph_block_ptr g a)
+      as H31
+      by (subst g'; apply lacv_heapgraph_block_ptr_old; assumption).
+    assert
+      (heapgraph_block_ptr g' (new_copied_v g to) = heapgraph_block_ptr g (new_copied_v g to))
+      as H32
+      by (subst g'; apply lacv_heapgraph_block_ptr_new; assumption).
+    rewrite <- H31.
+    rewrite <- H32 in H30.
+    assert
+      (writable_share (heapgraph_generation_sh g' (addr_gen a)))
+      as H33
+      by (unfold heapgraph_generation_sh; apply generation_sh__writable).
+    assert
+      (heapgraph_has_block g' (new_copied_v g to))
+      as H34
+      by (subst g'; apply lacv_heapgraph_has_block_new; assumption).
+    sep_apply (graph_rep_valid_int_or_ptr _ _ H34).
+    Intros.
+    rewrite <- H30 in H35.
+    assert
+      (heapgraph_has_block g' a)
+      as H36
+      by (subst g'; apply lgraph_add_copied_v__heapgraph_has_block; assumption).
+    remember (heapgraph_generation_sh g' (addr_gen a)) as sh'.
+    sep_apply (graph_vertex_lmc_ramif g' a (new_copied_v g to) H36).
+    rewrite <- Heqsh'.
+    Intros.
+    freeze [1; 2] FR1.
+    unfold vertex_rep, vertex_at.
+    Intros.
+    sep_apply (data_at_minus1_address sh' (Z2val (heapgraph_block_header g' a)) (heapgraph_block_ptr g' a)).
+    Intros.
+    forward.
+    clear H37.
+    try rewrite Int.signed_repr by rep_lia.
+    sep_apply (field_at_data_at_cancel
+                  sh' (if Archi.ptr64 then tulong else tuint)
+                  (if Archi.ptr64 then (Vlong (Int64.repr 0)) else (vint 0))
+                  (offset_val (- WORD_SIZE) (heapgraph_block_ptr g' a))).
+    forward_call (nv).
+    remember
+      (heapgraph_block_cells_vals g' a)
+      as l' eqn:Heql'.
+    assert
+      (0 < Zlength l')
+      as H37.
+    {
+      subst l'. rewrite fields_eq_length.
+      apply (proj1 (block_fields__range (heapgraph_block g' a))).
+    }
+    rewrite data_at_tarray_value_split_1 by assumption.
+    Intros.
+    assert_PROP (
+      force_val (sem_add_ptr_int int_or_ptr_type Signed (heapgraph_block_ptr g' a) (vint 0))
+      = field_address int_or_ptr_type [] (heapgraph_block_ptr g' a))
+      as H38.
+    {
+      clear. entailer!. unfold field_address. rewrite if_true by assumption.
+      simpl. rewrite isptr_offset_val_zero. 1: reflexivity.
+      destruct H7 ; try assumption.
+    }
+    forward.
+    clear H38.
+    sep_apply (field_at_data_at_cancel sh' int_or_ptr_type nv (heapgraph_block_ptr g' a)).
+    gather_SEP
+      (data_at _ (if Archi.ptr64 then tulong else tuint) _ _)
+      (data_at _ int_or_ptr_type nv _)
+      (data_at _ _ _ _).
+    rewrite H30.
+    subst l'.
+    rewrite <- lmc_vertex_rep_eq.
+    thaw FR1.
+    gather_SEP (vertex_rep _ _ _) (_ -* _).
+    sep_apply
+      (wand_frame_elim
+          (vertex_rep sh' (lgraph_mark_copied g' a (new_copied_v g to)) a)
+          (graph_rep (lgraph_mark_copied g' a (new_copied_v g to)))).
+    rewrite <- (lmc_heapgraph_block_ptr g' a (new_copied_v g to)) in *.
+    subst g'.
+    change
+      (lgraph_mark_copied (lgraph_add_copied_v g a to) a (new_copied_v g to))
+      with (lgraph_copy_v g a to)
+      in *.
+    remember
+      (lgraph_copy_v g a to)
+      as g' eqn:Heqg'.
+    rewrite <- H30 in *.
+    thaw FR.
+    forward_call (nv).
+    subst p_addr.
+    remember
+      (cut_thread_info t_info (Z.of_nat to) (heapgraph_block_size g a) Hi Hh)
+      as t_info' eqn:Heqt_info'.
+    unfold thread_info_rep.
+    Intros.
+    forward.
+    remember
+      (Znth z (live_roots_indices f_info))
+      as lz eqn:Heqlz.
+    gather_SEP
+      (data_at sh thread_info_type _ ti)
+      (heap_struct_rep sh _ _)
+      (heap_rest_rep _ ).
+    replace_SEP 0 (thread_info_rep sh (update_thread_info_arg t_info' lz nv H16) ti).
+    {
+      unfold thread_info_rep. simpl heap_head. simpl ti_heap_p.
+      simpl ti_args. simpl ti_heap. clear Heqt_info'. entailer!.
+    }
+    remember
+      (update_thread_info_arg t_info' lz nv H16)
+      as t eqn:Heqt.
+    subst t_info'.
+    rename t into t_info'.
+    rewrite H30 in H32.
+    assert
+      (forward_relation from to 0 (inl (inr a)) g g')
+      as H38
+      by (subst g'; constructor; assumption).
+    assert
+      (forward_condition g' t_info' from to)
+      as H39.
+    {
+      subst g' t_info' from. apply lcv_forward_condition; try assumption.
+      red. intuition.
+    }
+    remember
+      (upd_bunch z f_info roots (inr (new_copied_v g to)))
+      as roots' eqn:Heqroots'.
+    assert
+      (super_compatible (g', t_info', roots') f_info outlier)
+      as H40.
+    {
+      subst g' t_info' roots' lz. rewrite H30, H32.
+      apply lcv_super_compatible; try assumption. red. intuition.
+    }
+    assert
+      (thread_info_relation t_info t_info')
+      as H41.
+    {
+      subst t_info'. split; [|split]; [reflexivity| |]; intros m.
+      - rewrite utiacti_gen_size. reflexivity.
+      - rewrite utiacti_space_base. reflexivity.
+    }
+    forward_if.
+    {
+      pose proof H41 as HH41.
+      destruct H41 as [H41 [H43 H44]].
+      replace
+        fp
+        with (heapgraph_generation_base g' from)
+        by (subst fp g'; apply lcv_gen_start; assumption).
+      replace
+        (offset_val fn (heapgraph_generation_base g' from))
+        with (limit_address g' t_info' from).
+      2: {
+        subst fn gn.
+        unfold limit_address.
+        f_equal.
+        f_equal.
+        rewrite <- H43, <- (thread_info_relation__space_remembered _ _ from HH41).
+        unfold nth_space.
+        now rewrite <- nth_Znth'.
+      }
+      replace
+        n_addr
+        with (next_address t_info' to)
+        by (subst n_addr; rewrite H41; reflexivity).
+      forward_for_simple_bound
+        n
+        (EX i: Z, EX g3: HeapGraph, EX t_info3: thread_info,
+        PROP (super_compatible (g3, t_info3, roots') f_info outlier;
+              forward_loop
+                from to (Z.to_nat (depth - 1))
+                (sublist 0 i (heapgraph_field_pairs g' (new_copied_v g to)))
+                g' g3;
+              forward_condition g3 t_info3 from to;
+              thread_info_relation t_info' t_info3)
+        LOCAL (temp _new nv;
+                temp _sz (if Archi.ptr64 then
+                            Vlong (Int64.repr n) else vint n);
+                temp _from_start (heapgraph_generation_base g3 from);
+                temp _from_limit (limit_address g3 t_info3 from);
+                temp _next (next_address t_info3 to);
+                temp _depth (vint depth))
+        SEP (all_string_constants rsh gv;
+              fun_info_rep rsh f_info fi;
+              outlier_rep outlier;
+              graph_rep g3;
+              thread_info_rep sh t_info3 ti))%assert.
+      {
+        pose proof (block_fields__range2 (heapgraph_block g a)).
+        simpl in H45.
+        now rewrite <- Heqn in H45.
+      }
+      {
+        Exists g' t_info'. autorewrite with sublist.
+        assert
+          (forward_loop from to (Z.to_nat (depth - 1)) [] g' g')
+          by constructor.
+        unfold thread_info_relation.
+        entailer!.
+      }
+      {
+        Intros.
+        assert
+          (heapgraph_has_gen g' to)
+          as H50
+          by (rewrite Heqg', <- lcv_graph_has_gen; assumption).
+        assert
+          (heapgraph_has_block g' (new_copied_v g to))
+          as H51
+          by (rewrite Heqg'; apply lcv_heapgraph_has_block_new; assumption).
+        forward_call (rsh, sh, gv, fi, ti, g3, t_info3, f_info, roots', outlier, from, to, depth - 1, (@inr Z _ (new_copied_v g to, i))).
+        {
+          apply prop_right.
+          simpl.
+          rewrite sub_repr, H30.
+          do 4 f_equal.
+          first [rewrite sem_add_pi_ptr_special' | rewrite sem_add_pl_ptr_special']; auto.
+          - simpl.
+            f_equal.
+            erewrite fl_heapgraph_block_ptr; eauto.
+            subst g'.
+            now apply heapgraph_has_block_in_closure.
+          - now rewrite <- H30.
+        }
+        {
+          split3; [| |split].
+          - apply (fl_heapgraph_has_block _ _ _ _ _ _ H50 H47 _ H51).
+          - erewrite <- fl_block_fields; eauto. subst g'.
+            unfold lgraph_copy_v. subst n.
+            now rewrite <- lmc_block_fields, lacv_vlabel_new.
+          - erewrite <- fl_block_mark; eauto. subst g' from.
+            rewrite lcv_vlabel_new. auto. assumption.
+          - simpl. lia.
+        }
+        Intros vret.
+        destruct vret as [[g4 t_info4] roots4].
+        simpl fst in *.
+        simpl snd in *.
+        Exists g4 t_info4.
+        simpl in H53.
+        subst roots4.
+        assert
+          (heapgraph_generation_base g3 from = heapgraph_generation_base g4 from)
+          as H53.
+        {
+          eapply fr_gen_start; eauto.
+          erewrite <- fl_graph_has_gen; eauto.
+        }
+        rewrite H53.
+        assert
+          (limit_address g3 t_info3 from = limit_address g4 t_info4 from)
+          as H57.
+        {
+          unfold limit_address. f_equal. 2: assumption. f_equal.
+          rewrite (thread_info_relation__space_remembered _ _ _ H56).
+          destruct H56 as [? [? _]].
+          now rewrite H57.
+        }
+        rewrite H57.
+        assert
+          (next_address t_info3 to = next_address t_info4 to)
+          as H58.
+        {
+          unfold next_address.
+          f_equal.
+          now destruct H56.
+        }
+        rewrite H58.
+        clear H53 H57 H58.
+        assert
+          (thread_info_relation t_info' t_info4)
+          by (now apply tir_trans with t_info3).
+        assert
+          (forward_loop
+            from to (Z.to_nat (depth - 1))
+            (sublist 0 (i + 1) (heapgraph_field_pairs g' (new_copied_v g to)))
+            g' g4)
+          as H57.
+        {
+          eapply forward_loop_add_tail_vpp; eauto.
+          subst n g' from.
+          rewrite lcv_vlabel_new; assumption.
+        }
+        entailer!.
+      }
+      Intros g3 t_info3.
+      assert
+        (thread_info_relation t_info t_info3)
+        as H49
+        by (apply tir_trans with t_info'; [split; [|split]|]; assumption).
+      rewrite sublist_all in H46.
+      clear Heqt.
+      2: {
+        rewrite Z.le_lteq.
+        right.
+        subst n g' from.
+        now rewrite heapgraph_field_pairs__Zlength, lcv_vlabel_new.
+      }
+      Opaque super_compatible.
+      Exists g3 t_info3 roots'.
+      entailer!.
+      simpl.
+      rewrite <- Heqroot, H21, if_true by reflexivity.
+      split; auto.
+      replace
+        (Z.to_nat depth)
+        with (S (Z.to_nat (depth - 1)))
+        by (rewrite <- Z2Nat.inj_succ; [f_equal|]; lia).
+      now constructor.
+    }
+    assert
+      (depth = 0)
+      as H43
+      by lia.
+    subst depth.
+    clear H42 Heqnv.
+    forward.
+    remember
+      (cut_thread_info t_info (Z.of_nat to) (heapgraph_block_size g a) Hi Hh)
+      as t eqn:Heqt0.
+    Exists
+      (lgraph_copy_v g a to)
+      (update_thread_info_arg t lz nv H16)
+      (upd_bunch z f_info roots (inr (new_copied_v g to))).
+    entailer!.
+    simpl.
+    rewrite <- Heqroot.
+    rewrite if_true by reflexivity.
+    now rewrite H21.
+  }
   (* p is Vtype * Z, ie located in graph *)
-  - destruct p as [v n]. destruct H0 as [? [? [? ?]]]. freeze [0; 1; 2; 4] FR.
+  destruct p as [v n]. destruct H0 as [? [? [? ?]]]. freeze [0; 1; 2; 4] FR.
+  localize [vertex_rep (heapgraph_generation_sh g (addr_gen v)) g v].
+  unfold vertex_rep, vertex_at. Intros.
+  assert_PROP (offset_val (WORD_SIZE * n) (heapgraph_block_ptr g v) =
+                field_address (tarray int_or_ptr_type
+                                      (Zlength (heapgraph_block_cells_vals g v)))
+                              [ArraySubsc n] (heapgraph_block_ptr g v)). {
+    entailer!. unfold field_address. rewrite if_true; [simpl; f_equal|].
+    clear -H20 H11; rewrite <- fields_eq_length in H11.
+    unfold field_compatible in *; simpl in *; intuition.
+  }
+  assert (readable_share (heapgraph_generation_sh g (addr_gen v))) by
+    apply writable_readable, generation_sh__writable.
+  assert (is_pointer_or_integer (Znth n (heapgraph_block_cells_vals g v))). {
+    pose proof (mfv_all_is_ptr_or_int g v H9 H10 H0). rewrite Forall_forall in H16.
+    apply H16, Znth_In. rewrite fields_eq_length. assumption. } forward.
+  gather_SEP (data_at _ _ _ _) (data_at _ _ _ _).
+  replace_SEP 0 (vertex_rep (heapgraph_generation_sh g (addr_gen v)) g v).
+  1: unfold vertex_rep, vertex_at; entailer!.
+  unlocalize [graph_rep g]. 1: apply graph_vertex_ramif_stable; assumption. thaw FR.
+  unfold heapgraph_block_cells_vals.
+  rewrite H12, Znth_map; [|rewrite heapgraph_block_cells_eq_length; assumption].
+  assert_PROP (valid_int_or_ptr (heapgraph_cell_val g (Znth n (heapgraph_block_cells g v)))). {
+    destruct (Znth n (heapgraph_block_cells g v)) eqn:?; [destruct s|].
+    - unfold heapgraph_cell_val; unfold odd_Z2val.
+      replace (2 * z + 1) with (z + z + 1) by lia.
+      entailer!. apply valid_int_or_ptr_ii1.
+    - unfold heapgraph_cell_val, outlier_rep.
+      apply in_gcptr_outlier with (gcptr:= g0) (outlier:=outlier) (n:=n) in H0;
+        try assumption.
+      apply (in_map single_outlier_rep outlier g0) in H0.
+      replace_SEP 3 (single_outlier_rep g0). {
+        clear -H0.
+        apply (list_in_map_inv single_outlier_rep) in H0; destruct H0 as [? [? ?]].
+        rewrite H.
+        apply (in_map single_outlier_rep) in H0.
+        destruct (log_normalize.fold_right_andp
+                    (map single_outlier_rep outlier)
+                    (single_outlier_rep x) H0).
+        rewrite H1. entailer!; now apply andp_left1.
+      }
+      sep_apply (single_outlier_rep_valid_int_or_ptr g0); entailer!.
+    - rename f into e. unfold heapgraph_cell_val.
+      unfold no_dangling_dst in H10.
+      apply H10 with (e:=e) in H0.
+      1: sep_apply (graph_rep_valid_int_or_ptr g (dst g e) H0); entailer!.
+      unfold heapgraph_block_fields; rewrite <- filter_sum_right_In_iff, <- Heqc.
+      now apply Znth_In; rewrite heapgraph_block_cells_eq_length. }
+  forward_call (heapgraph_cell_val g (Znth n (heapgraph_block_cells g v))).
+  remember (graph_rep g * heap_rest_rep (ti_heap t_info) * outlier_rep outlier) as P.
+  pose proof (graph_and_heap_rest_data_at_ _ _ _ H7 H).
+  unfold generation_data_at_ in H18. remember (heapgraph_generation_base g from) as fp.
+  remember (heapgraph_generation_sh g from) as fsh.
+  remember
+    (gen_size t_info from - space_remembered (nth_space t_info from))
+    as gn.
+  remember (WORD_SIZE * gn)%Z as fn.
+  assert (P |-- (weak_derives P (memory_block fsh fn fp * TT) && emp) * P).
+  {
+    apply weak_derives_strong.
+    subst.
+    sep_apply H18.
+    rewrite data_at__memory_block.
+    unfold gen_size.
+    pose proof (space_remembered__order (nth_space t_info from)) as H19.
+    rewrite sizeof_tarray_int_or_ptr ; try lia.
+    entailer!.
+  }
+  destruct (Znth n (heapgraph_block_cells g v)) eqn:? ; [destruct s|].
+  (* Z + GC_Pointer + EType *)
+  {
+    (* Z *)
+    unfold heapgraph_cell_val, odd_Z2val. forward_if.
+    1: exfalso; apply H20'; reflexivity.
+    forward. Exists g t_info roots. entailer!. split.
+    * easy.
+    * unfold forward_condition, thread_info_relation.
+      simpl. rewrite Heqc, H12. simpl. constructor; [constructor|easy].
+  }
+  {
+    (* GC_Pointer *)
+    destruct g0. unfold heapgraph_cell_val, GC_Pointer2val. forward_if.
+    2: exfalso; apply Int.one_not_zero; assumption.
+    forward_call (Vptr b i). 
+    unfold thread_info_rep; Intros.
+    gather_SEP (graph_rep _) (heap_rest_rep _) (outlier_rep _).
+    rewrite <- HeqP. destruct H5.
+    replace_SEP 0 ((weak_derives P (memory_block fsh fn fp * TT) && emp) * P) by
+        (entailer; assumption). clear H19. Intros.
+    assert (P |-- (weak_derives P (valid_pointer (Vptr b i) * TT) && emp) * P). {
+      subst; cancel; apply andp_right; [|cancel].
+      assert (HS: emp |-- TT) by entailer; sep_apply HS; clear HS.
+      apply derives_weak. assert (In (GCPtr b i) outlier) by
+          (eapply in_gcptr_outlier; eauto).
+      sep_apply (outlier_rep_valid_pointer outlier (GCPtr b i) H19).
+      simpl GC_Pointer2val. cancel. }
+    replace_SEP 1 ((weak_derives P (valid_pointer (Vptr b i) * TT) && emp) * P) by (entailer; assumption).
+    Intros.
+    clear H19.
+    forward_call (fsh, fp, fn, (Vptr b i), P).
+    Intros vret.
+    destruct vret. (* is_from? *)
+    {
+      (* yes *)
+      rewrite HeqP. Intros.
+      gather_SEP (graph_rep _) (heap_rest_rep _).
+      sep_apply H18. rewrite Heqfn in v0.
+      pose proof in_gcptr_outlier g (GCPtr b i) outlier n v H0 H6 H11 Heqc.
+      sep_apply (outlier_rep_single_rep outlier (GCPtr b i)).
+      Intros.
+      gather_SEP (data_at_ _ _ _) (single_outlier_rep _).
+      change (Vptr b i) with (GC_Pointer2val (GCPtr b i)) in v0.
+      pose proof (generation_sh__writable (heapgraph_generation g from)).
+      change (generation_sh (heapgraph_generation g from)) with (heapgraph_generation_sh g from) in H22.
+      rewrite <- Heqfsh in H22. unfold generation_data_at_.
+      sep_apply (single_outlier_rep_memory_block_FF (GCPtr b i) fp gn fsh H22 v0).
+      assert_PROP False by entailer!. contradiction.
+    }
+    {
+      (* no *)
+      forward_if. 1: exfalso; apply H19'; reflexivity.
+      forward. Exists g t_info roots. entailer!.
+      - split3.
+        + unfold roots_compatible. easy.
+        + simpl. rewrite Heqc, H12. simpl. constructor.
+        + easy.
+      - unfold thread_info_rep. entailer!.
+    }
+  }
+  (* EType *)
+  rename f into e.
+  unfold heapgraph_cell_val. remember (dst g e) as v'.
+  assert (isptr (heapgraph_block_ptr g v')). { (**)
+    unfold heapgraph_block_ptr; unfold offset_val.
+    remember (addr_gen v') as n'.
+    assert (heapgraph_has_block g v'). {
+      unfold no_dangling_dst in H10.
+      subst. clear -H0 H10 H11 e Heqc.
+      apply (H10 v H0).
+      unfold heapgraph_block_fields;
+      rewrite <- filter_sum_right_In_iff, <- Heqc; apply Znth_In.
+      now rewrite heapgraph_block_cells_eq_length.
+    }
+    pose proof (heapgraph_has_block__has_gen H20) as Hgen.
+    rewrite <- Heqn' in Hgen.
+    pose proof (heapgraph_generation_base__isptr g n' Hgen).
+    destruct (heapgraph_generation_base g n'); try contradiction; auto.
+  }
+  destruct (heapgraph_block_ptr g v') eqn:?; try contradiction.
+  forward_if. 2: exfalso; apply Int.one_not_zero in H21; assumption.
+  clear H21 H21'. forward_call (Vptr b i).
+  unfold thread_info_rep; Intros.
+  gather_SEP (graph_rep _) (heap_rest_rep _) (outlier_rep _).
+  rewrite <- HeqP.
+  replace_SEP 0
+              ((weak_derives P (memory_block fsh fn fp * TT) && emp) * P) by
+      (entailer; assumption).
+  clear H19. Intros. assert (heapgraph_has_block g v'). { (**)
+    rewrite Heqv'.
+    unfold no_dangling_dst in H10.
+    clear -H10 H0 e Heqc H11. apply (H10 v H0).
+    unfold heapgraph_block_fields.
+    rewrite <- filter_sum_right_In_iff.
+    rewrite <- Heqc.
+    apply Znth_In.
+    rewrite heapgraph_block_cells_eq_length; assumption.
+  }
+  assert (P |-- (weak_derives P (valid_pointer (Vptr b i) * TT) && emp) * P). {
+    apply weak_derives_strong. subst.
+    remember (dst g e) as v'.
+    sep_apply (graph_rep_vertex_rep g v' H19).
+    Intros shh. unfold vertex_rep, vertex_at. rewrite Heqv0.
+    sep_apply (data_at_valid_ptr
+                  shh (tarray int_or_ptr_type (Zlength (heapgraph_block_cells_vals g v')))
+                  (heapgraph_block_cells_vals g v') (Vptr b i)).
+    - apply readable_nonidentity, writable_readable_share; assumption.
+    - simpl. rewrite fields_eq_length.
+      pose proof (proj1 (block_fields__range (heapgraph_block g v'))). rewrite Z.max_r; lia.
+    - cancel.
+  }
+  replace_SEP 1 (weak_derives P (valid_pointer (Vptr b i) * TT) && emp * P)
+    by entailer!. clear H21. Intros.
+  forward_call (fsh, fp, fn, (Vptr b i), P).
+  (* is_from *)
+  Intros vv. rewrite HeqP.
+  sep_apply (graph_and_heap_rest_v_in_range_iff _ _ _ _ H H7 H19).
+  Intros. rewrite <- Heqfp, <- Heqgn, <- Heqfn, Heqv0 in H21.
+  destruct vv.
+  2: {
+    forward_if.
+    {
+      exfalso.
+      now apply H22'.
+    }
+    rewrite H21 in n0.
+    forward.
+    Exists g t_info roots.
+    entailer!; simpl.
+    2: {
+      unfold thread_info_rep.
+      entailer!.
+    }
+    rewrite H12, Heqc.
+    simpl.
+    Transparent super_compatible.
+    unfold super_compatible.
+    split ; auto.
+    split; [|split].
+    + constructor; auto.
+    + constructor; auto.
+    + apply tir_id.
+  }
+  (* yes, is_from *)
+  rewrite H21 in v0.
+  clear H21.
+  forward_if.
+  2: {
+    exfalso.
+    now inversion H21.
+  }
+  freeze [1; 2; 3; 4; 5; 6] FR.
+  clear H21 H21'. localize [vertex_rep (heapgraph_generation_sh g (addr_gen v')) g v'].
+  unfold vertex_rep, vertex_at. Intros. rewrite v0.
+  assert (readable_share (heapgraph_generation_sh g from)) by
+      (unfold heapgraph_generation_sh; apply writable_readable, generation_sh__writable).
+  rewrite <- Heqv0.
+  sep_apply (data_at_minus1_address
+                (heapgraph_generation_sh g from) (Z2val (heapgraph_block_header g v')) (heapgraph_block_ptr g v')).
+  Intros. forward. clear H22.
+  gather_SEP (data_at _ _ _ _) (data_at _ _ _ _).
+  replace_SEP 0 (vertex_rep (heapgraph_generation_sh g (addr_gen v')) g v') by
+      (unfold vertex_rep, vertex_at; entailer!).
+  unlocalize [graph_rep g]. 1: apply (graph_vertex_ramif_stable _ _ H19).
+  forward_if.
+  {
+    (* yes, already forwarded *)
+    try apply Int64.same_if_eq in H22.
+    pose proof (heapgraph_block_header__repr_iff g v'). simpl in H23.
+    rewrite H23 in H22. clear H23.
+    localize [vertex_rep (heapgraph_generation_sh g (addr_gen v')) g v'].
+    rewrite v0. unfold vertex_rep, vertex_at. Intros.
+    unfold heapgraph_block_cells_vals at 2. rewrite H22.
+    assert (0 <= 0 < Zlength (heapgraph_block_cells_vals g v')). {
+        split. 1: lia. rewrite fields_eq_length.
+        apply (proj1 (block_fields__range (heapgraph_block g v'))).
+    }
+    assert (is_pointer_or_integer (heapgraph_block_ptr g (block_copied_vertex (heapgraph_block g v')))).
+    {
+      apply isptr_is_pointer_or_integer. unfold heapgraph_block_ptr.
+      rewrite isptr_offset_val.
+      apply heapgraph_generation_base__isptr, H9; assumption.
+    }
+    forward.
+    rewrite Znth_0_cons.
+    gather_SEP (data_at _ _ _ _) (data_at _ _ _ _).
+    replace_SEP 0 (vertex_rep (heapgraph_generation_sh g (addr_gen v')) g v').
+    {
+      unfold vertex_rep, vertex_at. unfold heapgraph_block_cells_vals at 3.
+      rewrite H22. entailer!.
+    }
+    unlocalize [graph_rep g]. 1: apply (graph_vertex_ramif_stable _ _ H19).
     localize [vertex_rep (heapgraph_generation_sh g (addr_gen v)) g v].
     unfold vertex_rep, vertex_at. Intros.
-    assert_PROP (offset_val (WORD_SIZE * n) (heapgraph_block_ptr g v) =
-                 field_address (tarray int_or_ptr_type
-                                       (Zlength (heapgraph_block_cells_vals g v)))
-                               [ArraySubsc n] (heapgraph_block_ptr g v)). {
-      entailer!. unfold field_address. rewrite if_true; [simpl; f_equal|].
-      clear -H20 H11; rewrite <- fields_eq_length in H11.
-      unfold field_compatible in *; simpl in *; intuition.
+    assert (writable_share (heapgraph_generation_sh g (addr_gen v))) by (unfold heapgraph_generation_sh; apply generation_sh__writable).
+    forward.
+    sep_apply (field_at_data_at_cancel
+                  (heapgraph_generation_sh g (addr_gen v))
+                  (tarray int_or_ptr_type (Zlength (heapgraph_block_cells_vals g v)))
+                  (upd_Znth n (heapgraph_block_cells_vals g v)
+                  (heapgraph_block_ptr g (block_copied_vertex (heapgraph_block g v'))))
+                  (heapgraph_block_ptr g v)).
+    gather_SEP (data_at _ _ _ _ ) (data_at _ _ _ _).
+    remember (block_copied_vertex (heapgraph_block g v')).
+    remember (labeledgraph_gen_dst g e a) as g'.
+    replace_SEP 0 (vertex_rep (heapgraph_generation_sh g' (addr_gen v)) g' v).
+    {
+      unfold vertex_rep, vertex_at.
+      replace (heapgraph_generation_sh g' (addr_gen v)) with
+          (heapgraph_generation_sh g (addr_gen v)) by (subst g'; reflexivity).
+      replace (Zlength (heapgraph_block_cells_vals g' v)) with
+          (Zlength (heapgraph_block_cells_vals g v)) by
+          (subst g'; repeat rewrite fields_eq_length;
+          apply lgd_raw_fld_length_eq).
+      rewrite (lgd_mfv_change_in_one_spot g v e a n);
+        [|rewrite heapgraph_block_cells_eq_length| | ]; try assumption.
+      entailer!.
     }
-    assert (readable_share (heapgraph_generation_sh g (addr_gen v))) by
-      apply writable_readable, generation_sh__writable.
-    assert (is_pointer_or_integer (Znth n (heapgraph_block_cells_vals g v))). {
-      pose proof (mfv_all_is_ptr_or_int g v H9 H10 H0). rewrite Forall_forall in H16.
-      apply H16, Znth_In. rewrite fields_eq_length. assumption. } forward.
-    gather_SEP (data_at _ _ _ _) (data_at _ _ _ _).
-    replace_SEP 0 (vertex_rep (heapgraph_generation_sh g (addr_gen v)) g v).
-    1: unfold vertex_rep, vertex_at; entailer!.
-    unlocalize [graph_rep g]. 1: apply graph_vertex_ramif_stable; assumption. thaw FR.
-    unfold heapgraph_block_cells_vals.
-    rewrite H12, Znth_map; [|rewrite heapgraph_block_cells_eq_length; assumption].
-    assert_PROP (valid_int_or_ptr (heapgraph_cell_val g (Znth n (heapgraph_block_cells g v)))). {
-      destruct (Znth n (heapgraph_block_cells g v)) eqn:?; [destruct s|].
-      - unfold heapgraph_cell_val; unfold odd_Z2val.
-        replace (2 * z + 1) with (z + z + 1) by lia.
-        entailer!. apply valid_int_or_ptr_ii1.
-      - unfold heapgraph_cell_val, outlier_rep.
-        apply in_gcptr_outlier with (gcptr:= g0) (outlier:=outlier) (n:=n) in H0;
-          try assumption.
-        apply (in_map single_outlier_rep outlier g0) in H0.
-        replace_SEP 3 (single_outlier_rep g0). {
-          clear -H0.
-          apply (list_in_map_inv single_outlier_rep) in H0; destruct H0 as [? [? ?]].
-          rewrite H.
-          apply (in_map single_outlier_rep) in H0.
-          destruct (log_normalize.fold_right_andp
-                     (map single_outlier_rep outlier)
-                     (single_outlier_rep x) H0).
-          rewrite H1. entailer!; now apply andp_left1.
-        }
-        sep_apply (single_outlier_rep_valid_int_or_ptr g0); entailer!.
-      - rename f into e. unfold heapgraph_cell_val.
-        unfold no_dangling_dst in H10.
-        apply H10 with (e:=e) in H0.
-        1: sep_apply (graph_rep_valid_int_or_ptr g (dst g e) H0); entailer!.
-        unfold heapgraph_block_fields; rewrite <- filter_sum_right_In_iff, <- Heqc.
-        now apply Znth_In; rewrite heapgraph_block_cells_eq_length. }
-    forward_call (heapgraph_cell_val g (Znth n (heapgraph_block_cells g v))).
-    remember (graph_rep g * heap_rest_rep (ti_heap t_info) * outlier_rep outlier) as P.
-    pose proof (graph_and_heap_rest_data_at_ _ _ _ H7 H).
-    unfold generation_data_at_ in H18. remember (heapgraph_generation_base g from) as fp.
-    remember (heapgraph_generation_sh g from) as fsh. remember (gen_size t_info from) as gn.
-    remember (WORD_SIZE * gn)%Z as fn.
-    assert (P |-- (weak_derives P (memory_block fsh fn fp * TT) && emp) * P). {
-      apply weak_derives_strong. subst. sep_apply H18.
-      rewrite data_at__memory_block.
-      rewrite sizeof_tarray_int_or_ptr; [Intros; cancel | unfold gen_size].
-      destruct (space_capacity__tight_range (nth_space t_info from)). assumption. }
-    destruct (Znth n (heapgraph_block_cells g v)) eqn:? ; [destruct s|].
-    (* Z + GC_Pointer + EType *)
-    + (* Z *)
-      unfold heapgraph_cell_val, odd_Z2val. forward_if.
-      1: exfalso; apply H20'; reflexivity.
-      forward. Exists g t_info roots. entailer!. split.
-      * easy.
-      * unfold forward_condition, thread_info_relation.
-        simpl. rewrite Heqc, H12. simpl. constructor; [constructor|easy].
-    + (* GC_Pointer *)
-      destruct g0. unfold heapgraph_cell_val, GC_Pointer2val. forward_if.
-      2: exfalso; apply Int.one_not_zero; assumption.
-      forward_call (Vptr b i). 
-      unfold thread_info_rep; Intros.
-      gather_SEP (graph_rep _) (heap_rest_rep _) (outlier_rep _).
-      rewrite <- HeqP. destruct H5.
-      replace_SEP 0 ((weak_derives P (memory_block fsh fn fp * TT) && emp) * P) by
-          (entailer; assumption). clear H19. Intros.
-      assert (P |-- (weak_derives P (valid_pointer (Vptr b i) * TT) && emp) * P). {
-        subst; cancel; apply andp_right; [|cancel].
-        assert (HS: emp |-- TT) by entailer; sep_apply HS; clear HS.
-        apply derives_weak. assert (In (GCPtr b i) outlier) by
-            (eapply in_gcptr_outlier; eauto).
-        sep_apply (outlier_rep_valid_pointer outlier (GCPtr b i) H19).
-        simpl GC_Pointer2val. cancel. }
-      replace_SEP 1 ((weak_derives P (valid_pointer (Vptr b i) * TT) && emp) * P) by
-          (entailer; assumption). Intros. clear H19.
-      forward_call (fsh, fp, fn, (Vptr b i), P).
+    subst g'; subst a.
+    unlocalize [graph_rep (labeledgraph_gen_dst g e
+                                                (block_copied_vertex (heapgraph_block g v')))].
+    1: apply (graph_vertex_lgd_ramif g v e (block_copied_vertex (heapgraph_block g v')) n);
+      try (rewrite heapgraph_block_cells_eq_length); assumption.
+    Exists (labeledgraph_gen_dst g e (block_copied_vertex (heapgraph_block g (dst g e))))
+            t_info roots.
+    entailer!.
+    2: unfold thread_info_rep; thaw FR; entailer!.
+    pose proof (lgd_no_dangling_dst_copied_vert g e (dst g e) H9 H19 H22 H10) as Hno_dangling_dst.
+    split; [|split; [|split; [|split]]]; try easy.
+    {
+      Transparent super_compatible.
+      unfold super_compatible.
+      unfold roots_compatible in *.
+      intuition idtac.
       {
-        entailer!.
-        simpl.
-        admit.
+        now apply lgd_graph_thread_info_compatible.
       }
-      Intros vret. destruct vret. (* is_from? *)
-      * (* yes *)
-        rewrite HeqP. Intros.
-        gather_SEP (graph_rep _) (heap_rest_rep _).
-        sep_apply H18. rewrite Heqfn in v0.
-        pose proof in_gcptr_outlier g (GCPtr b i) outlier n v H0 H6 H11 Heqc.
-        sep_apply (outlier_rep_single_rep outlier (GCPtr b i)).
-        Intros.
-        gather_SEP (data_at_ _ _ _) (single_outlier_rep _).
-        change (Vptr b i) with (GC_Pointer2val (GCPtr b i)) in v0.
-        pose proof (generation_sh__writable (heapgraph_generation g from)).
-        change (generation_sh (heapgraph_generation g from)) with (heapgraph_generation_sh g from) in H22.
-        rewrite <- Heqfsh in H22. unfold generation_data_at_.
-        sep_apply (single_outlier_rep_memory_block_FF (GCPtr b i) fp gn fsh H22 v0).
-        assert_PROP False by entailer!. contradiction.
-      * (* no *)
-        forward_if. 1: exfalso; apply H19'; reflexivity.
-        forward. Exists g t_info roots. entailer!.
-        -- split3.
-           ++ unfold roots_compatible. easy.
-           ++ simpl. rewrite Heqc, H12. simpl. constructor.
-           ++ easy.
-        -- unfold thread_info_rep. entailer!.
-    + (* EType *)
-      rename f into e.
-      unfold heapgraph_cell_val. remember (dst g e) as v'.
-      assert (isptr (heapgraph_block_ptr g v')). { (**)
-        unfold heapgraph_block_ptr; unfold offset_val.
-        remember (addr_gen v') as n'.
-        assert (heapgraph_has_block g v'). {
-          unfold no_dangling_dst in H10.
-          subst. clear -H0 H10 H11 e Heqc.
-          apply (H10 v H0).
-          unfold heapgraph_block_fields;
-          rewrite <- filter_sum_right_In_iff, <- Heqc; apply Znth_In.
-          now rewrite heapgraph_block_cells_eq_length.
-        }
-        pose proof (heapgraph_has_block__has_gen H20) as Hgen.
-        rewrite <- Heqn' in Hgen.
-        pose proof (heapgraph_generation_base__isptr g n' Hgen).
-        destruct (heapgraph_generation_base g n'); try contradiction; auto.
-      }
-      destruct (heapgraph_block_ptr g v') eqn:?; try contradiction.
-      forward_if. 2: exfalso; apply Int.one_not_zero in H21; assumption.
-      clear H21 H21'. forward_call (Vptr b i).
-      unfold thread_info_rep; Intros.
-      gather_SEP (graph_rep _) (heap_rest_rep _) (outlier_rep _).
-      rewrite <- HeqP.
-      replace_SEP 0
-                  ((weak_derives P (memory_block fsh fn fp * TT) && emp) * P) by
-          (entailer; assumption).
-      clear H19. Intros. assert (heapgraph_has_block g v'). { (**)
-        rewrite Heqv'.
-        unfold no_dangling_dst in H10.
-        clear -H10 H0 e Heqc H11. apply (H10 v H0).
-        unfold heapgraph_block_fields.
-        rewrite <- filter_sum_right_In_iff.
-        rewrite <- Heqc.
-        apply Znth_In.
-        rewrite heapgraph_block_cells_eq_length; assumption.
-      }
-      assert (P |-- (weak_derives P (valid_pointer (Vptr b i) * TT) && emp) * P). {
-        apply weak_derives_strong. subst.
-        remember (dst g e) as v'.
-        sep_apply (graph_rep_vertex_rep g v' H19).
-        Intros shh. unfold vertex_rep, vertex_at. rewrite Heqv0.
-        sep_apply (data_at_valid_ptr
-                     shh (tarray int_or_ptr_type (Zlength (heapgraph_block_cells_vals g v')))
-                     (heapgraph_block_cells_vals g v') (Vptr b i)).
-        - apply readable_nonidentity, writable_readable_share; assumption.
-        - simpl. rewrite fields_eq_length.
-          pose proof (proj1 (block_fields__range (heapgraph_block g v'))). rewrite Z.max_r; lia.
-        - cancel.
-      }
-      replace_SEP 1 (weak_derives P (valid_pointer (Vptr b i) * TT) && emp * P)
-        by entailer!. clear H21. Intros.
-      forward_call (fsh, fp, fn, (Vptr b i), P).
       {
-        entailer!.
-        simpl.
-        admit.
+        now apply lgd_rgc.
       }
-      (* is_from *)
-      Intros vv. rewrite HeqP.
-      sep_apply (graph_and_heap_rest_v_in_range_iff _ _ _ _ H H7 H19).
-      Intros. rewrite <- Heqfp, <- Heqgn, <- Heqfn, Heqv0 in H21. destruct vv.
-      * (* yes, is_from *)
-        rewrite H21 in v0. clear H21. forward_if.
-        2: exfalso; inversion H21.
-        freeze [1; 2; 3; 4; 5; 6] FR.
-        clear H21 H21'. localize [vertex_rep (heapgraph_generation_sh g (addr_gen v')) g v'].
-        unfold vertex_rep, vertex_at. Intros. rewrite v0.
-        assert (readable_share (heapgraph_generation_sh g from)) by
-            (unfold heapgraph_generation_sh; apply writable_readable, generation_sh__writable).
-        rewrite <- Heqv0.
-        sep_apply (data_at_minus1_address
-                     (heapgraph_generation_sh g from) (Z2val (heapgraph_block_header g v')) (heapgraph_block_ptr g v')).
-        Intros. forward. clear H22.
-        gather_SEP (data_at _ _ _ _) (data_at _ _ _ _).
-        replace_SEP 0 (vertex_rep (heapgraph_generation_sh g (addr_gen v')) g v') by
-            (unfold vertex_rep, vertex_at; entailer!).
-        unlocalize [graph_rep g]. 1: apply (graph_vertex_ramif_stable _ _ H19).
-        forward_if.
-        -- (* yes, already forwarded *)
-          try apply Int64.same_if_eq in H22.
-          pose proof (heapgraph_block_header__repr_iff g v'). simpl in H23.
-          rewrite H23 in H22. clear H23.
-          localize [vertex_rep (heapgraph_generation_sh g (addr_gen v')) g v'].
-          rewrite v0. unfold vertex_rep, vertex_at. Intros.
-          unfold heapgraph_block_cells_vals at 2. rewrite H22.
-          assert (0 <= 0 < Zlength (heapgraph_block_cells_vals g v')). {
-             split. 1: lia. rewrite fields_eq_length.
-             apply (proj1 (block_fields__range (heapgraph_block g v'))).
-          }
-          assert (is_pointer_or_integer (heapgraph_block_ptr g (block_copied_vertex (heapgraph_block g v')))).
-          {
-            apply isptr_is_pointer_or_integer. unfold heapgraph_block_ptr.
-            rewrite isptr_offset_val.
-            apply heapgraph_generation_base__isptr, H9; assumption.
-          }
-          forward.
-          rewrite Znth_0_cons.
-          gather_SEP (data_at _ _ _ _) (data_at _ _ _ _).
-          replace_SEP 0 (vertex_rep (heapgraph_generation_sh g (addr_gen v')) g v').
-          {
-            unfold vertex_rep, vertex_at. unfold heapgraph_block_cells_vals at 3.
-            rewrite H22. entailer!.
-          }
-          unlocalize [graph_rep g]. 1: apply (graph_vertex_ramif_stable _ _ H19).
-          localize [vertex_rep (heapgraph_generation_sh g (addr_gen v)) g v].
-          unfold vertex_rep, vertex_at. Intros.
-          assert (writable_share (heapgraph_generation_sh g (addr_gen v))) by (unfold heapgraph_generation_sh; apply generation_sh__writable).
-          forward.
-          sep_apply (field_at_data_at_cancel
-                       (heapgraph_generation_sh g (addr_gen v))
-                       (tarray int_or_ptr_type (Zlength (heapgraph_block_cells_vals g v)))
-                       (upd_Znth n (heapgraph_block_cells_vals g v)
-                       (heapgraph_block_ptr g (block_copied_vertex (heapgraph_block g v'))))
-                       (heapgraph_block_ptr g v)).
-          gather_SEP (data_at _ _ _ _ ) (data_at _ _ _ _).
-          remember (block_copied_vertex (heapgraph_block g v')).
-          remember (labeledgraph_gen_dst g e a) as g'.
-          replace_SEP 0 (vertex_rep (heapgraph_generation_sh g' (addr_gen v)) g' v).
-          1: { unfold vertex_rep, vertex_at.
-               replace (heapgraph_generation_sh g' (addr_gen v)) with
-                   (heapgraph_generation_sh g (addr_gen v)) by (subst g'; reflexivity).
-               replace (Zlength (heapgraph_block_cells_vals g' v)) with
-                   (Zlength (heapgraph_block_cells_vals g v)) by
-                   (subst g'; repeat rewrite fields_eq_length;
-                    apply lgd_raw_fld_length_eq).
-               rewrite (lgd_mfv_change_in_one_spot g v e a n);
-                 [|rewrite heapgraph_block_cells_eq_length| | ]; try assumption.
-               entailer!. }
-          subst g'; subst a.
-          unlocalize [graph_rep (labeledgraph_gen_dst g e
-                                                      (block_copied_vertex (heapgraph_block g v')))].
-          1: apply (graph_vertex_lgd_ramif g v e (block_copied_vertex (heapgraph_block g v')) n);
-            try (rewrite heapgraph_block_cells_eq_length); assumption.
-          Exists (labeledgraph_gen_dst g e (block_copied_vertex (heapgraph_block g (dst g e))))
-                 t_info roots.
-          entailer!.
-          2: unfold thread_info_rep; thaw FR; entailer!.
-          pose proof (lgd_no_dangling_dst_copied_vert g e (dst g e) H9 H19 H22 H10) as Hno_dangling_dst.
-          split; [|split; [|split; [|split]]]; try easy.
-          ++ unfold super_compatible.
-             unfold roots_compatible in *.
-             admit.
-(* 
-             intuition idtac.
-             {
-               now apply lgd_forall_heapgraph_has_block.
-             }
-             {
-              unfold outlier_compatible in *.
-              unfold roots_outlier_compatible in *.
-              unfold roots_graph_compatible in *.
-              unfold no_dangling_dst in Hno_dangling_dst.
-              intros x Hx z Hz.
-              apply lgd_heapgraph_has_block in Hx.
-              now apply (H6 x).
-             }
- *)
-          ++ simpl forward_p2forward_t.
-             rewrite H12, Heqc.
-             now constructor.
-          ++ unfold forward_condition.
-             apply (lgd_copy_compatible g (block_copied_vertex (heapgraph_block g (dst g e))) e) in H9.
-             intuition idtac.
-        -- (* not yet forwarded *)
-           forward. thaw FR.  freeze [0; 1; 2; 3; 4; 5] FR.
-           try apply Int64_eq_false in H22.
-           pose proof (heapgraph_block_header__repr_iff g v'). simpl in H23.
-           rewrite H23 in H22. clear H23. apply not_true_is_false in H22.
-           rewrite heapgraph_block_header__Wosize by assumption.
-           assert (0 <= Z.of_nat to < 12). {
-             clear -H H8. destruct H as [_ [_ ?]]. red in H8.
-             pose proof (heap_spaces__size (ti_heap t_info)).
-             rewrite Zlength_correct in H0. rep_lia. } unfold heap_struct_rep.
-           destruct (gt_gs_compatible _ _ H _ H8) as [H24 H25 H26 HH27].
-           simpl in H24, H25, H26, HH27.
-           rewrite nth_space_Znth in *.
-           remember (Znth (Z.of_nat to) (heap_spaces (ti_heap t_info))) as sp_to.
-           assert (isptr (space_base sp_to)) by (rewrite <- H24; apply generation_base__isptr).
-           remember (map space_tri (heap_spaces (ti_heap t_info))).
-           assert (@Znth (val * (val * (val * val))) (Vundef, (Vundef, (Vundef, Vundef)))
-                         (Z.of_nat to) l = space_tri sp_to). {
-             subst l sp_to. rewrite Znth_map by (rewrite heap_spaces__size; rep_lia).
-             reflexivity. }
-           forward; rewrite H28; unfold space_tri. 1: entailer!.
-           forward. simpl sem_binary_operation'.
-           rewrite sapi_ptr_val; [| assumption | rep_lia].
-           Opaque Znth. forward. Transparent Znth.
-           rewrite sapil_ptr_val by easy. rewrite H28. unfold space_tri.
-           rewrite <- Z.add_assoc.
-           replace (1 + Zlength (block_fields (heapgraph_block g v'))) with (heapgraph_block_size g v') by
-               (unfold heapgraph_block_size; lia). thaw FR. freeze [0; 2; 3; 4; 5; 6] FR.
-           assert (Hi : 0 <= Z.of_nat to < Zlength (heap_spaces (ti_heap t_info))) by
-               (rewrite heap_spaces__size; rep_lia).
-           assert (Hh: has_space (Znth (Z.of_nat to) (heap_spaces (ti_heap t_info)))
-                                 (heapgraph_block_size g v')). {
-             red. split. 1: pose proof (heapgraph_block_size__one g v'); lia.
-             transitivity (unmarked_gen_size g (addr_gen v')).
-             - apply single_unmarked_le; assumption.
-             - red in H1. unfold rest_gen_size in H1. subst from.
-               rewrite nth_space_Znth in H1.
-               lia.
-          }
-           assert (Hn: space_base (Znth (Z.of_nat to) (heap_spaces (ti_heap t_info))) <>
-                       nullval). {
-             rewrite <- Heqsp_to. destruct (space_base sp_to); try contradiction.
-             intro Hn. inversion Hn. }
-           rewrite (heap_rest_rep_cut
-                      (ti_heap t_info) (Z.of_nat to) (heapgraph_block_size g v') Hi Hh Hn).
-           rewrite <- Heqsp_to. thaw FR.
-           gather_SEP (data_at _ _ _ ti) (data_at _ _ _ _) (heap_rest_rep _).
-           replace_SEP 0 (thread_info_rep
-                            sh (cut_thread_info t_info _ _ Hi Hh) ti). {
-             entailer. unfold thread_info_rep. simpl ti_heap. simpl ti_heap_p. cancel.
-             simpl heap_spaces. rewrite <- upd_Znth_map. unfold cut_space.
-             unfold space_tri at 3. simpl. unfold heap_struct_rep. cancel. }
-           sep_apply (graph_vertex_ramif_stable _ _ H19). Intros.
-           freeze [1; 2; 3; 4; 5] FR. rewrite v0.
-           remember (heapgraph_generation_sh g from) as shv.
-           assert (writable_share (space_sh sp_to)) by
-               (rewrite <- H25; apply generation_sh__writable).
-           remember (space_sh sp_to) as sht.
-           rewrite (data_at__tarray_value _ _ 1). 2: unfold heapgraph_block_size; rep_lia.
-           Intros.
-           remember (offset_val (WORD_SIZE * space_allocated sp_to) (space_base sp_to)).
-           rewrite (data_at__int_or_ptr_integer sht v1).
-           assert_PROP
-             (force_val (sem_add_ptr_int
-                           (if Archi.ptr64 then tulong else tuint) Signed
-                           (offset_val (WORD_SIZE * (space_allocated sp_to + 1))
-                                       (space_base sp_to))
-                           (eval_unop Oneg tint (vint 1))) =
-              field_address (if Archi.ptr64 then tulong else tuint) [] v1). {
-             subst v1. entailer!. unfold field_address.
-             simpl. rewrite neg_repr. rewrite sem_add_pi_ptr_special; auto. 2: rep_lia.
-             rewrite if_true by assumption. simpl. rewrite !offset_offset_val.
-             f_equal. unfold WORD_SIZE. lia. }
-           forward. sep_apply (field_at_data_at_cancel
-                                 sht (if Archi.ptr64 then tulong else tuint)
-                                 (Z2val (heapgraph_block_header g v')) v1). clear H30.
-           subst v1. rewrite offset_offset_val.
-           replace (heapgraph_block_size g v' - 1) with (Zlength (block_fields (heapgraph_block g v')))
-             by (unfold heapgraph_block_size; lia).
-           replace (WORD_SIZE * space_allocated sp_to + WORD_SIZE * 1) with
-               (WORD_SIZE * (space_allocated sp_to + 1))%Z by rep_lia.
-           remember (offset_val (WORD_SIZE * (space_allocated sp_to + 1))
-                                (space_base sp_to)) as nv.
-           thaw FR. freeze [0; 1; 2; 3; 4; 5] FR. rename i into j.
-           remember (Zlength (block_fields (heapgraph_block g v'))) as n'.
-           assert (isptr nv) by (subst nv; rewrite isptr_offset_val; assumption).
-           remember (field_address heap_type
-                                   [StructField _next; ArraySubsc (Z.of_nat to);
-                                    StructField _spaces] (ti_heap_p t_info)) as n_addr.
-           forward_for_simple_bound
-             n'
-             (EX i: Z,
-              PROP ( )
-              LOCAL (temp _new nv;
-                     temp _sz (if Archi.ptr64 then Vlong (Int64.repr n') else vint n');
-                     temp _v (heapgraph_block_ptr g v');
-                     temp _from_start fp;
-                     temp _from_limit (offset_val fn fp);
-                     temp _next n_addr;
-                     temp _p (offset_val (WORD_SIZE * n) (heapgraph_block_ptr g v));
-                     temp _depth (vint depth))
-              SEP (vertex_rep shv g v';
-                   data_at sht (tarray int_or_ptr_type i)
-                           (sublist 0 i (heapgraph_block_cells_vals g v')) nv;
-                   data_at_ sht (tarray int_or_ptr_type (n' - i))
-                            (offset_val (WORD_SIZE * i) nv); FRZL FR))%assert.
-           ++ pose proof (block_fields__range2 (heapgraph_block g v')). simpl in H31.
-              now rewrite <- Heqn' in H31.
-           ++ rewrite sublist_nil. replace (n' - 0) with n' by lia.
-              replace (WORD_SIZE * 0)%Z with 0 by lia.
-              rewrite isptr_offset_val_zero by assumption.
-              rewrite data_at_zero_array_eq; [entailer! | easy..].
-              admit.
-           ++ unfold vertex_rep, vertex_at. Intros.
-              rewrite fields_eq_length, <- Heqn'. forward.
-              ** entailer!. pose proof (mfv_all_is_ptr_or_int _ _ H9 H10 H19) as HH.
-                 rewrite Forall_forall in HH.
-                 apply HH, Znth_In.
-                 now rewrite fields_eq_length.
-              ** rewrite (data_at__tarray_value _ _ 1) by lia. Intros.
-                 rewrite data_at__singleton_array_eq.
-                 assert_PROP
-                   (field_compatible int_or_ptr_type []
-                                     (offset_val (WORD_SIZE * i) nv)) by
-                     (sep_apply (data_at__local_facts
-                                   sht int_or_ptr_type
-                                   (offset_val (WORD_SIZE * i) nv)); entailer!).
-                 assert_PROP
-                   ((if Archi.ptr64 then
-                      force_val (sem_add_ptr_long int_or_ptr_type
-                                                  nv (Vlong (Int64.repr i)))
-                     else force_val (sem_add_ptr_int int_or_ptr_type
-                                                     Signed nv (vint i))) =
-                    field_address int_or_ptr_type []
-                                  (offset_val (WORD_SIZE * i) nv)). {
-                   unfold field_address. rewrite if_true by assumption.
-                   clear. entailer!. } simpl in H33.
-                 gather_SEP (data_at shv _ _ _)
-                            (data_at _ (_ n') _ _).
-                 replace_SEP 0 (vertex_rep shv g v') by
-                     (unfold vertex_rep, vertex_at;
-                      rewrite fields_eq_length; entailer!). forward.
-                 rewrite offset_offset_val.
-                 replace (n' - i - 1) with (n' - (i + 1)) by lia.
-                 replace (WORD_SIZE * i + WORD_SIZE * 1) with
-                     (WORD_SIZE * (i + 1))%Z by rep_lia.
-                 gather_SEP (data_at _ _ _ nv) (field_at _ _ _ _ _).
-                 rewrite data_at_mfs_eq;
-                                   [entailer! | assumption | subst n'; assumption].
-           ++ thaw FR. rewrite v0, <- Heqshv.
-              gather_SEP (vertex_rep _ _ _) (_ -* _).
-              replace_SEP 0 (graph_rep g) by (entailer!; apply wand_frame_elim).
-              rewrite sublist_all by (rewrite fields_eq_length; lia).
-              replace_SEP 2 emp. {
-                replace (n' - n') with 0 by lia. clear. entailer.
-                apply data_at__value_0_size. }
-              assert (nv = heapgraph_block_ptr g (new_copied_v g to)). {
-                subst nv. unfold heapgraph_block_ptr. unfold new_copied_v. simpl. f_equal.
-                - unfold heapgraph_block_offset. simpl. rewrite H26. reflexivity.
-                - unfold heapgraph_generation_base. rewrite if_true by assumption.
-                  rewrite H24. reflexivity. }
-              gather_SEP (data_at sht _ _ nv) (emp) (data_at sht _ _ _).
-              replace_SEP
-                0 (vertex_at (heapgraph_generation_sh g to)
-                             (heapgraph_block_ptr g (new_copied_v g to))
-                             (heapgraph_block_header g v') (heapgraph_block_cells_vals g v')). {
-                normalize. rewrite <- H25.
-                change (generation_sh (heapgraph_generation g to)) with (heapgraph_generation_sh g to).
-                rewrite <- fields_eq_length in Heqn'.
-                replace (offset_val (WORD_SIZE * space_allocated sp_to) (space_base sp_to))
-                  with (offset_val (- WORD_SIZE) nv) by
-                    (rewrite Heqnv; rewrite offset_offset_val; f_equal; rep_lia).
-                rewrite <- H31. unfold vertex_at; entailer!. }
-              gather_SEP (vertex_at _ _ _ _) (graph_rep _).
-              rewrite (copied_v_derives_new_g g v' to) by assumption.
-              freeze [1; 2; 3; 4] FR. remember (lgraph_add_copied_v g v' to) as g'.
-              assert (heapgraph_block_ptr g' v' = heapgraph_block_ptr g v') by
-                  (subst g'; apply lacv_heapgraph_block_ptr_old; assumption).
-              assert (heapgraph_block_ptr g' (new_copied_v g to) =
-                      heapgraph_block_ptr g (new_copied_v g to)) by
-                  (subst g'; apply lacv_heapgraph_block_ptr_new; assumption).
-              rewrite <- H32. rewrite <- H33 in H31.
-              assert (writable_share (heapgraph_generation_sh g' (addr_gen v'))) by
-                  (unfold heapgraph_generation_sh; apply generation_sh__writable).
-              assert (heapgraph_has_block g' (new_copied_v g to)) by
-                  (subst g'; apply lacv_heapgraph_has_block_new; assumption).
-              sep_apply (graph_rep_valid_int_or_ptr _ _ H35). Intros.
-              rewrite <- H31 in H36. assert (heapgraph_has_block g' v') by
-                  (subst g'; apply lgraph_add_copied_v__heapgraph_has_block; assumption).
-              remember (heapgraph_generation_sh g' (addr_gen v')) as sh'.
-              sep_apply (graph_vertex_lmc_ramif g' v' (new_copied_v g to) H37).
-              rewrite <- Heqsh'. Intros. freeze [1; 2] FR1.
-              unfold vertex_rep, vertex_at. Intros.
-              sep_apply (data_at_minus1_address
-                           sh' (Z2val (heapgraph_block_header g' v')) (heapgraph_block_ptr g' v')).
-              Intros. forward. clear H38.
-              sep_apply (field_at_data_at_cancel
-                           sh' (if Archi.ptr64 then tulong else tuint) (Z2val 0)
-                           (offset_val (- WORD_SIZE) (heapgraph_block_ptr g' v'))).
-              forward_call (nv). remember (heapgraph_block_cells_vals g' v') as l'.
-              assert (0 < Zlength l'). {
-                subst l'. rewrite fields_eq_length.
-                apply (proj1 (block_fields__range (heapgraph_block g' v'))). }
-              rewrite data_at_tarray_value_split_1 by assumption. Intros.
-              assert_PROP (force_val (sem_add_ptr_int int_or_ptr_type Signed
-                                                      (heapgraph_block_ptr g' v') (vint 0))
-                           =
-                           field_address int_or_ptr_type [] (heapgraph_block_ptr g' v')).
-              {
-                clear. entailer!. unfold field_address. rewrite if_true by assumption.
-                simpl. rewrite isptr_offset_val_zero. 1: reflexivity.
-                now destruct H7.
-              }
-              forward. clear H39.
-              sep_apply (field_at_data_at_cancel
-                           sh' int_or_ptr_type nv (heapgraph_block_ptr g' v')).
-              gather_SEP (data_at sh' (if Archi.ptr64 then tulong else tuint) _ _)
-                         (data_at sh' int_or_ptr_type _ _) (data_at _ _ _ _).
-              rewrite H31. subst l'.
-              rewrite <- lmc_vertex_rep_eq.
-              thaw FR1.
-              gather_SEP (vertex_rep _ _ _) (_ -* _).
-              sep_apply
-                (wand_frame_elim
-                   (vertex_rep sh' (lgraph_mark_copied g' v' (new_copied_v g to)) v')
-                   (graph_rep (lgraph_mark_copied g' v' (new_copied_v g to)))).
-              rewrite <- (lmc_heapgraph_block_ptr g' v' (new_copied_v g to)) in *. subst g'.
-              change (lgraph_mark_copied
-                        (lgraph_add_copied_v g v' to) v' (new_copied_v g to))
-                with (lgraph_copy_v g v' to) in *.
-              remember (lgraph_copy_v g v' to) as g'.
-
-              assert (heapgraph_block_ptr g' v' = heapgraph_block_ptr g v') by
-              (subst g'; apply lcv_heapgraph_block_ptr_old; assumption).
-              assert (heapgraph_block_ptr g' (new_copied_v g to) =
-                      heapgraph_block_ptr g (new_copied_v g to)) by
-                  (subst g'; apply lcv_heapgraph_block_ptr_new; assumption).
-              assert (writable_share (heapgraph_generation_sh g' (addr_gen v'))) by
-                  (unfold heapgraph_generation_sh; apply generation_sh__writable).
-              assert (heapgraph_has_block g' (new_copied_v g to)) by
-                  (subst g'; apply lcv_heapgraph_has_block_new; assumption).
-              forward_call (nv).
-              rewrite <- H31 in *.
-              rewrite lacv_heapgraph_block_ptr;
-                [|apply heapgraph_has_block_in_closure|]; try assumption.
-              rewrite <- H32.
-              rewrite <- (lcv_heapgraph_block_ptr g v' to v);
-                try rewrite <- (lcv_heapgraph_block_ptr g v' to v) in H14;
-                try apply heapgraph_has_block_in_closure; try assumption.
-              rewrite (lcv_mfv_Zlen_eq g v v' to H8 H0) in H14. rewrite <- Heqg' in *.
-              remember (heapgraph_generation_sh g' (addr_gen v)) as shh.
-              remember (heapgraph_block_cells_vals g' v) as mfv.
-              remember (new_copied_v g to).
-              remember (labeledgraph_gen_dst g' e a) as g1.
-              assert (0 <= n < Zlength (heapgraph_block_cells_vals g' v)) by
-                  (subst g'; rewrite fields_eq_length, <- lcv_block_fields; assumption).
-              assert (Znth n (heapgraph_block_cells g' v) = inr e) by
-                  (subst g'; unfold heapgraph_block_cells in *;
-                   rewrite <- lcv_block_fields; assumption).
-              assert (0 <= n < Zlength (heapgraph_block_cells g' v)) by
-                  (rewrite heapgraph_block_cells_eq_length;
-                   rewrite fields_eq_length in H43; assumption).
-              assert (heapgraph_has_block g' v) by
-                  (subst g'; apply lcv_heapgraph_has_block_old; assumption).
-              assert (v <> v') by
-                  (intro; subst v; clear -v0 H13; lia).
-              assert (block_mark (heapgraph_block g' v) = false) by
-                (subst g'; rewrite <- lcv_block_mark; assumption).
-              assert (writable_share shh) by
-                  (rewrite Heqshh; unfold heapgraph_generation_sh; apply generation_sh__writable).
-              localize [vertex_rep (heapgraph_generation_sh g' (addr_gen v)) g' v].
-              unfold vertex_rep, vertex_at. Intros.
-              rewrite Heqmfv in *; rewrite <- Heqshh.
-              forward.
-              rewrite H31.
-              sep_apply (field_at_data_at_cancel
-                           shh
-                           (tarray int_or_ptr_type (Zlength (heapgraph_block_cells_vals g' v)))
-                           (upd_Znth n (heapgraph_block_cells_vals g' v) (heapgraph_block_ptr g' a))
-                           (heapgraph_block_ptr g' v)).
-              gather_SEP (data_at shh _ _ _) (data_at shh _ _ _).
-              replace_SEP 0 (vertex_rep (heapgraph_generation_sh g1 (addr_gen v)) g1 v).
-              1: { unfold vertex_rep, vertex_at.
-                   replace (heapgraph_generation_sh g1 (addr_gen v)) with shh by
-                       (subst shh g1; reflexivity).
-                   replace (Zlength (heapgraph_block_cells_vals g1 v)) with
-                       (Zlength (heapgraph_block_cells_vals g' v)) by
-                       (subst g1; repeat rewrite fields_eq_length;
-                        apply lgd_raw_fld_length_eq).
-                   rewrite (lgd_mfv_change_in_one_spot g' v e a n);
-                     try assumption. entailer!. }
-              subst g1; subst a.
-              unlocalize [graph_rep (labeledgraph_gen_dst g' e (new_copied_v g to))].
-              1: apply (graph_vertex_lgd_ramif g' v e (new_copied_v g to) n);
-                assumption.
-              remember (new_copied_v g to) as v1.
-              remember (labeledgraph_gen_dst g' e v1) as g1.
-              thaw FR.
-              remember (cut_thread_info t_info (Z.of_nat to) (heapgraph_block_size g v') Hi Hh)
-                as t_info'.
-              unfold thread_info_rep. Intros.
-              assert (0 <= 0 < Zlength (ti_args t_info')) by
-                  (rewrite arg_size; rep_lia).
-              gather_SEP
-                (data_at _ _ _ _)
-                (heap_struct_rep _ _ _)
-                (heap_rest_rep _).
-              replace_SEP 0 (thread_info_rep sh t_info' ti).
-              { unfold thread_info_rep. simpl heap_head. simpl ti_heap_p.
-                simpl ti_args. simpl ti_heap. entailer!. }
-              rewrite H31 in H33.
-                assert (forward_relation from to 0 (inr e) g g1) by
-                    (subst g1 g' v1 v'; constructor; assumption).
-                assert (In e (heapgraph_block_fields g v)). { (**)
-                  unfold heapgraph_block_fields.
-                  rewrite <- filter_sum_right_In_iff.
-                  rewrite <- Heqc.
-                  apply (Znth_In n (heapgraph_block_cells g v)).
-                  rewrite heapgraph_block_cells_eq_length. assumption.
-                }
-                assert (forward_condition g1 t_info' from to). {
-                  subst g1 g' t_info' from v'.
-                  assert (heapgraph_has_block (lgraph_copy_v g (dst g e) to) (dst g e)) as HH.
-                  {
-                    destruct H37 ; now constructor.
-                  }
-                  apply lgd_forward_condition; try assumption.
-                  apply lcv_forward_condition_unchanged; try assumption.
-                  red. intuition. }
-                remember roots as roots'.
-                assert (super_compatible (g1, t_info', roots') f_info outlier). {
-                  subst g1 g' t_info' roots'.
-                  apply lgd_super_compatible, lcv_super_compatible_unchanged;
-                    try assumption.
-                  red; intuition. }
-              assert (thread_info_relation t_info t_info'). {
-                subst t_info'. split; [|split]; [reflexivity| |]; intros m.
-                - rewrite cti_gen_size. reflexivity.
-                - rewrite cti_space_base. reflexivity. }
-                forward_if.
-              ** destruct H55 as [? [? ?]]. replace fp with (heapgraph_generation_base g1 from) by
-                     (subst fp g1 g'; apply lcv_gen_start; assumption).
-                 replace
-                    (offset_val fn (heapgraph_generation_base g1 from)) with
-                    (limit_address g1 t_info' from).
-                 2: {
-                  subst fn gn.
-                  rewrite H57.
-                  admit.
-                 }
-                 replace n_addr with (next_address t_info' to) by
-                     (subst n_addr; rewrite H55; reflexivity).
-                 forward_for_simple_bound
-                   n'
-                   (EX i: Z, EX g3: HeapGraph, EX t_info3: thread_info,
-                    PROP (super_compatible (g3, t_info3, roots') f_info outlier;
-                          forward_loop
-                            from to (Z.to_nat (depth - 1))
-                            (sublist 0 i (heapgraph_field_pairs g1 (new_copied_v g to)))
-                            g1 g3;
-                          forward_condition g3 t_info3 from to;
-                          thread_info_relation t_info' t_info3)
-                    LOCAL (temp _new nv;
-                           temp _sz (if Archi.ptr64 then Vlong (Int64.repr n')
-                                     else vint n');
-                           temp _from_start (heapgraph_generation_base g3 from);
-                           temp _from_limit (limit_address g3 t_info3 from);
-                           temp _next (next_address t_info3 to);
-                           temp _depth (vint depth))
-                    SEP (all_string_constants rsh gv;
-                         fun_info_rep rsh f_info fi;
-                         outlier_rep outlier;
-                         graph_rep g3;
-                         thread_info_rep sh t_info3 ti))%assert.
-                 --- pose proof (block_fields__range2 (heapgraph_block g v')). simpl in H59.
-                     now rewrite <- Heqn' in H59.
-                 --- Exists g1 t_info'. autorewrite with sublist.
-                     assert (forward_loop from to (Z.to_nat (depth - 1)) [] g1 g1) by
-                         constructor. unfold thread_info_relation.
-                     destruct H54 as [? [? [? ?]]].
-                     entailer!. easy.
-                 --- Intros.
-                     assert (heapgraph_has_gen g1 to) by
-                         (rewrite Heqg1, lgd_graph_has_gen; subst g';
-                          rewrite <- lcv_graph_has_gen; assumption).
-                     assert (heapgraph_has_block g1 (new_copied_v g to)) by
-                       (subst g1; rewrite <- lgd_heapgraph_has_block;
-                       rewrite Heqg'; apply lcv_heapgraph_has_block_new; assumption).
-                     forward_call (rsh, sh, gv, fi, ti, g3, t_info3, f_info, roots',
-                                   outlier, from, to, depth - 1,
-                                   (@inr Z _ (new_copied_v g to, i))).
-                     +++ apply prop_right. simpl. rewrite sub_repr.
-                         do 4 f_equal. rewrite H31.
-                         first [rewrite sem_add_pi_ptr_special' |
-                                rewrite sem_add_pl_ptr_special']; auto.
-                         *** simpl. f_equal.
-                             rewrite <- (lgd_heapgraph_block_ptr_eq g' e v1), <- Heqg1.
-                             subst v1. apply (fl_heapgraph_block_ptr _ _ _ _ _ _ H64 H61).
-                             apply heapgraph_has_block_in_closure; assumption.
-                         *** rewrite <- H31. assumption.
-                     +++ split3; [| |split].
-                         *** destruct H53 as [_ [_ [? _]]].
-                             apply (fl_heapgraph_has_block _ _ _ _ _ _ H64 H61 _ H65).
-                         *** erewrite <- fl_block_fields; eauto. subst g1.
-                             unfold lgraph_copy_v. subst n'.
-                             rewrite <- lgd_raw_fld_length_eq.
-                             subst g'. rewrite lcv_vlabel_new.
-                             assumption. rewrite v0. lia.
-                         *** erewrite <- fl_block_mark; eauto. subst g1 from.
-                             rewrite <- lgd_block_mark_eq. subst g'.
-                             rewrite lcv_vlabel_new; try assumption.
-                         *** simpl; lia.
-                     +++ Intros vret. destruct vret as [[g4 t_info4] roots4].
-                         simpl fst in *. simpl snd in *. Exists g4 t_info4.
-                         simpl in H67. subst roots4.
-                         assert (heapgraph_generation_base g3 from = heapgraph_generation_base g4 from). {
-                           eapply fr_gen_start; eauto.
-                           erewrite <- fl_graph_has_gen; eauto. } rewrite H67.
-                         assert (limit_address g3 t_info3 from =
-                                 limit_address g4 t_info4 from). {
-                           unfold limit_address. f_equal. 2: assumption. f_equal.
-                           rewrite (thread_info_relation__space_remembered _ _ _ H70).
-                           destruct H70 as [_ [H71 _]].
-                           now rewrite H71.
-                          }
-                         rewrite H71.
-                         assert (next_address t_info3 to = next_address t_info4 to). {
-                           unfold next_address. f_equal. destruct H70. assumption. }
-                         rewrite H72. clear H67 H71 H72.
-                         assert (thread_info_relation t_info' t_info4) by
-                             (apply tir_trans with t_info3; assumption).
-                         assert (forward_loop
-                                   from to (Z.to_nat (depth - 1))
-                                   (sublist 0 (i + 1)
-                                            (heapgraph_field_pairs g1 (new_copied_v g to)))
-                                   g1 g4). {
-                            eapply forward_loop_add_tail_vpp; eauto. subst n' g1 from.
-                           rewrite <- lgd_raw_fld_length_eq. subst g'.
-                           rewrite lcv_vlabel_new; assumption. }
-                         entailer!.
-                 --- Intros g3 t_info3.
-                     assert (thread_info_relation t_info t_info3) by
-                         (apply tir_trans with t_info';
-                          [split; [| split]|]; assumption).
-                     rewrite sublist_all in H60.
-                     2: { rewrite Z.le_lteq. right. subst n' g1 from.
-                          rewrite heapgraph_field_pairs__Zlength,  <- lgd_raw_fld_length_eq.
-                          subst g'; rewrite lcv_vlabel_new; auto. }
-                     Opaque super_compatible. Exists g3 t_info3 roots.
-                     entailer!. simpl.
-                     replace (Z.to_nat depth) with (S (Z.to_nat (depth - 1))) by
-                         (rewrite <- Z2Nat.inj_succ; [f_equal|]; lia).
-                     rewrite Heqc, H12. simpl.
-                     constructor; [reflexivity | assumption..].
-                     Transparent super_compatible.
-              ** assert (depth = 0) by lia. subst depth. clear H56.
-                 deadvars!. clear Heqnv. forward.
-                 Exists g1 t_info' roots. entailer!. simpl. rewrite Heqc.
-                 simpl field2forward. rewrite H12. simpl. now constructor.
-      * forward_if. 1: exfalso; apply H22'; reflexivity.
-        rewrite H21 in n0. forward.
-        Exists g t_info roots. entailer!; simpl.
-        -- rewrite H12, Heqc. simpl. split; auto. split; [|split].
-           ++ constructor. auto.
-           ++ split; auto.
-           ++ apply tir_id.
-        -- unfold thread_info_rep. entailer!.
-Admitted.
+      {
+        intros x Hx z Hz.
+        apply lgd_heapgraph_has_block in Hx.
+        now apply (H6 x).
+      }
+    }
+    {
+      simpl forward_p2forward_t.
+      rewrite H12, Heqc.
+      now constructor.
+    }
+    {
+      unfold forward_condition.
+      apply (lgd_copy_compatible g (block_copied_vertex (heapgraph_block g (dst g e))) e) in H9.
+      intuition idtac.
+    }
+  }
+  (* not yet forwarded *)
+    forward. thaw FR.  freeze [0; 1; 2; 3; 4; 5] FR.
+    try apply Int64_eq_false in H22.
+    pose proof (heapgraph_block_header__repr_iff g v'). simpl in H23.
+    rewrite H23 in H22. clear H23. apply not_true_is_false in H22.
+    rewrite heapgraph_block_header__Wosize by assumption.
+    assert (0 <= Z.of_nat to < 12). {
+      clear -H H8. destruct H as [_ [_ ?]]. red in H8.
+      pose proof (heap_spaces__size (ti_heap t_info)).
+      rewrite Zlength_correct in H0. rep_lia. } unfold heap_struct_rep.
+    destruct (gt_gs_compatible _ _ H _ H8) as [H24 H25 H26 HH27].
+    simpl in H24, H25, H26, HH27.
+    rewrite nth_space_Znth in *.
+    remember (Znth (Z.of_nat to) (heap_spaces (ti_heap t_info))) as sp_to.
+    assert (isptr (space_base sp_to)) by (rewrite <- H24; apply generation_base__isptr).
+    remember (map space_tri (heap_spaces (ti_heap t_info))).
+    assert (@Znth (val * (val * (val * val))) (Vundef, (Vundef, (Vundef, Vundef)))
+                  (Z.of_nat to) l = space_tri sp_to). {
+      subst l sp_to. rewrite Znth_map by (rewrite heap_spaces__size; rep_lia).
+      reflexivity. }
+    forward; rewrite H28; unfold space_tri. 1: entailer!.
+    forward. simpl sem_binary_operation'.
+    rewrite sapi_ptr_val; [| assumption | rep_lia].
+    Opaque Znth. forward. Transparent Znth.
+    rewrite sapil_ptr_val by easy. rewrite H28. unfold space_tri.
+    rewrite <- Z.add_assoc.
+    replace (1 + Zlength (block_fields (heapgraph_block g v'))) with (heapgraph_block_size g v') by
+        (unfold heapgraph_block_size; lia). thaw FR. freeze [0; 2; 3; 4; 5; 6] FR.
+    assert (Hi : 0 <= Z.of_nat to < Zlength (heap_spaces (ti_heap t_info))) by
+        (rewrite heap_spaces__size; rep_lia).
+    assert (Hh: has_space (Znth (Z.of_nat to) (heap_spaces (ti_heap t_info)))
+                          (heapgraph_block_size g v')). {
+      red. split. 1: pose proof (heapgraph_block_size__one g v'); lia.
+      transitivity (unmarked_gen_size g (addr_gen v')).
+      - apply single_unmarked_le; assumption.
+      - red in H1. unfold rest_gen_size in H1. subst from.
+        rewrite nth_space_Znth in H1.
+        lia.
+  }
+  assert (Hn: space_base (Znth (Z.of_nat to) (heap_spaces (ti_heap t_info))) <>
+              nullval). {
+    rewrite <- Heqsp_to. destruct (space_base sp_to); try contradiction.
+    intro Hn. inversion Hn. }
+  rewrite (heap_rest_rep_cut
+            (ti_heap t_info) (Z.of_nat to) (heapgraph_block_size g v') Hi Hh Hn).
+  rewrite <- Heqsp_to. thaw FR.
+  gather_SEP (data_at _ _ _ ti) (data_at _ _ _ _) (heap_rest_rep _).
+  replace_SEP 0 (thread_info_rep
+                  sh (cut_thread_info t_info _ _ Hi Hh) ti). {
+    entailer. unfold thread_info_rep. simpl ti_heap. simpl ti_heap_p. cancel.
+    simpl heap_spaces. rewrite <- upd_Znth_map. unfold cut_space.
+    unfold space_tri at 3. simpl. unfold heap_struct_rep. cancel. }
+  sep_apply (graph_vertex_ramif_stable _ _ H19). Intros.
+  freeze [1; 2; 3; 4; 5] FR. rewrite v0.
+  remember (heapgraph_generation_sh g from) as shv.
+  assert (writable_share (space_sh sp_to)) by
+      (rewrite <- H25; apply generation_sh__writable).
+  remember (space_sh sp_to) as sht.
+  rewrite (data_at__tarray_value _ _ 1). 2: unfold heapgraph_block_size; rep_lia.
+  Intros.
+  remember (offset_val (WORD_SIZE * space_allocated sp_to) (space_base sp_to)).
+  rewrite (data_at__int_or_ptr_integer sht v1).
+  assert_PROP
+    (force_val (sem_add_ptr_int
+                  (if Archi.ptr64 then tulong else tuint) Signed
+                  (offset_val (WORD_SIZE * (space_allocated sp_to + 1))
+                              (space_base sp_to))
+                  (eval_unop Oneg tint (vint 1))) =
+    field_address (if Archi.ptr64 then tulong else tuint) [] v1). {
+    subst v1. entailer!. unfold field_address.
+    simpl. rewrite neg_repr. rewrite sem_add_pi_ptr_special; auto. 2: rep_lia.
+    rewrite if_true by assumption. simpl. rewrite !offset_offset_val.
+    f_equal. unfold WORD_SIZE. lia. }
+  forward. sep_apply (field_at_data_at_cancel
+                        sht (if Archi.ptr64 then tulong else tuint)
+                        (Z2val (heapgraph_block_header g v')) v1). clear H30.
+  subst v1. rewrite offset_offset_val.
+  replace (heapgraph_block_size g v' - 1) with (Zlength (block_fields (heapgraph_block g v')))
+    by (unfold heapgraph_block_size; lia).
+  replace (WORD_SIZE * space_allocated sp_to + WORD_SIZE * 1) with
+      (WORD_SIZE * (space_allocated sp_to + 1))%Z by rep_lia.
+  remember (offset_val (WORD_SIZE * (space_allocated sp_to + 1))
+                      (space_base sp_to)) as nv.
+  thaw FR. freeze [0; 1; 2; 3; 4; 5] FR. rename i into j.
+  remember (Zlength (block_fields (heapgraph_block g v'))) as n'.
+  assert (isptr nv) by (subst nv; rewrite isptr_offset_val; assumption).
+  remember (field_address heap_type
+                          [StructField _next; ArraySubsc (Z.of_nat to);
+                          StructField _spaces] (ti_heap_p t_info)) as n_addr.
+  forward_for_simple_bound
+    n'
+    (EX i: Z,
+    PROP ( )
+    LOCAL (temp _new nv;
+            temp _sz (if Archi.ptr64 then Vlong (Int64.repr n') else vint n');
+            temp _v (heapgraph_block_ptr g v');
+            temp _from_start fp;
+            temp _from_limit (offset_val fn fp);
+            temp _next n_addr;
+            temp _p (offset_val (WORD_SIZE * n) (heapgraph_block_ptr g v));
+            temp _depth (vint depth))
+    SEP (vertex_rep shv g v';
+          data_at sht (tarray int_or_ptr_type i)
+                  (sublist 0 i (heapgraph_block_cells_vals g v')) nv;
+          data_at_ sht (tarray int_or_ptr_type (n' - i))
+                  (offset_val (WORD_SIZE * i) nv); FRZL FR))%assert.
+  {
+    pose proof (block_fields__range2 (heapgraph_block g v')).
+    simpl in H31.
+    now rewrite <- Heqn' in H31.
+  }
+  {
+    rewrite sublist_nil. replace (n' - 0) with n' by lia.
+    replace (WORD_SIZE * 0)%Z with 0 by lia.
+    rewrite isptr_offset_val_zero by assumption.
+    rewrite data_at_zero_array_eq; [entailer! | easy..].
+  }
+  {
+    unfold vertex_rep, vertex_at. Intros.
+    rewrite fields_eq_length, <- Heqn'. forward.
+    ** entailer!. pose proof (mfv_all_is_ptr_or_int _ _ H9 H10 H19) as HH.
+        rewrite Forall_forall in HH.
+        apply HH, Znth_In.
+        now rewrite fields_eq_length.
+    ** rewrite (data_at__tarray_value _ _ 1) by lia. Intros.
+        rewrite data_at__singleton_array_eq.
+        assert_PROP
+          (field_compatible int_or_ptr_type []
+                            (offset_val (WORD_SIZE * i) nv)) by
+            (sep_apply (data_at__local_facts
+                          sht int_or_ptr_type
+                          (offset_val (WORD_SIZE * i) nv)); entailer!).
+        assert_PROP
+          ((if Archi.ptr64 then
+            force_val (sem_add_ptr_long int_or_ptr_type
+                                        nv (Vlong (Int64.repr i)))
+            else force_val (sem_add_ptr_int int_or_ptr_type
+                                            Signed nv (vint i))) =
+          field_address int_or_ptr_type []
+                        (offset_val (WORD_SIZE * i) nv)). {
+          unfold field_address. rewrite if_true by assumption.
+          clear. entailer!. } simpl in H33.
+        gather_SEP (data_at shv _ _ _)
+                  (data_at _ (_ n') _ _).
+        replace_SEP 0 (vertex_rep shv g v') by
+            (unfold vertex_rep, vertex_at;
+            rewrite fields_eq_length; entailer!). forward.
+        rewrite offset_offset_val.
+        replace (n' - i - 1) with (n' - (i + 1)) by lia.
+        replace (WORD_SIZE * i + WORD_SIZE * 1) with
+            (WORD_SIZE * (i + 1))%Z by rep_lia.
+        gather_SEP (data_at _ _ _ nv) (field_at _ _ _ _ _).
+        rewrite data_at_mfs_eq;
+                          [entailer! | assumption | subst n'; assumption].
+  }
+  thaw FR. rewrite v0, <- Heqshv.
+  gather_SEP (vertex_rep _ _ _) (_ -* _).
+  replace_SEP 0 (graph_rep g) by (entailer!; apply wand_frame_elim).
+  rewrite sublist_all by (rewrite fields_eq_length; lia).
+  replace_SEP 2 emp. {
+    replace (n' - n') with 0 by lia. clear. entailer.
+    apply data_at__value_0_size. }
+  assert (nv = heapgraph_block_ptr g (new_copied_v g to)). {
+    subst nv. unfold heapgraph_block_ptr. unfold new_copied_v. simpl. f_equal.
+    - unfold heapgraph_block_offset. simpl. rewrite H26. reflexivity.
+    - unfold heapgraph_generation_base. rewrite if_true by assumption.
+      rewrite H24. reflexivity. }
+  gather_SEP (data_at sht _ _ nv) (emp) (data_at sht _ _ _).
+  replace_SEP
+    0 (vertex_at (heapgraph_generation_sh g to)
+                  (heapgraph_block_ptr g (new_copied_v g to))
+                  (heapgraph_block_header g v') (heapgraph_block_cells_vals g v')). {
+    normalize. rewrite <- H25.
+    change (generation_sh (heapgraph_generation g to)) with (heapgraph_generation_sh g to).
+    rewrite <- fields_eq_length in Heqn'.
+    replace (offset_val (WORD_SIZE * space_allocated sp_to) (space_base sp_to))
+      with (offset_val (- WORD_SIZE) nv) by
+        (rewrite Heqnv; rewrite offset_offset_val; f_equal; rep_lia).
+    rewrite <- H31. unfold vertex_at; entailer!. }
+  gather_SEP (vertex_at _ _ _ _) (graph_rep _).
+  rewrite (copied_v_derives_new_g g v' to) by assumption.
+  freeze [1; 2; 3; 4] FR. remember (lgraph_add_copied_v g v' to) as g'.
+  assert (heapgraph_block_ptr g' v' = heapgraph_block_ptr g v') by
+      (subst g'; apply lacv_heapgraph_block_ptr_old; assumption).
+  assert (heapgraph_block_ptr g' (new_copied_v g to) =
+          heapgraph_block_ptr g (new_copied_v g to)) by
+      (subst g'; apply lacv_heapgraph_block_ptr_new; assumption).
+  rewrite <- H32. rewrite <- H33 in H31.
+  assert (writable_share (heapgraph_generation_sh g' (addr_gen v'))) by
+      (unfold heapgraph_generation_sh; apply generation_sh__writable).
+  assert (heapgraph_has_block g' (new_copied_v g to)) by
+      (subst g'; apply lacv_heapgraph_has_block_new; assumption).
+  sep_apply (graph_rep_valid_int_or_ptr _ _ H35). Intros.
+  rewrite <- H31 in H36. assert (heapgraph_has_block g' v') by
+      (subst g'; apply lgraph_add_copied_v__heapgraph_has_block; assumption).
+  remember (heapgraph_generation_sh g' (addr_gen v')) as sh'.
+  sep_apply (graph_vertex_lmc_ramif g' v' (new_copied_v g to) H37).
+  rewrite <- Heqsh'. Intros. freeze [1; 2] FR1.
+  unfold vertex_rep, vertex_at. Intros.
+  sep_apply (data_at_minus1_address
+                sh' (Z2val (heapgraph_block_header g' v')) (heapgraph_block_ptr g' v')).
+  Intros. forward. clear H38.
+  sep_apply (field_at_data_at_cancel
+                sh' (if Archi.ptr64 then tulong else tuint) (Z2val 0)
+                (offset_val (- WORD_SIZE) (heapgraph_block_ptr g' v'))).
+  forward_call (nv). remember (heapgraph_block_cells_vals g' v') as l'.
+  assert (0 < Zlength l'). {
+    subst l'. rewrite fields_eq_length.
+    apply (proj1 (block_fields__range (heapgraph_block g' v'))). }
+  rewrite data_at_tarray_value_split_1 by assumption. Intros.
+  assert_PROP (
+    force_val (sem_add_ptr_int int_or_ptr_type Signed (heapgraph_block_ptr g' v') (vint 0))
+    = field_address int_or_ptr_type [] (heapgraph_block_ptr g' v')).
+  {
+    clear. entailer!. unfold field_address. rewrite if_true by assumption.
+    simpl. rewrite isptr_offset_val_zero. 1: reflexivity.
+    now destruct H7.
+  }
+  forward. clear H39.
+  sep_apply (field_at_data_at_cancel
+                sh' int_or_ptr_type nv (heapgraph_block_ptr g' v')).
+  gather_SEP (data_at sh' (if Archi.ptr64 then tulong else tuint) _ _)
+              (data_at sh' int_or_ptr_type _ _) (data_at _ _ _ _).
+  rewrite H31. subst l'.
+  rewrite <- lmc_vertex_rep_eq.
+  thaw FR1.
+  gather_SEP (vertex_rep _ _ _) (_ -* _).
+  sep_apply
+    (wand_frame_elim
+        (vertex_rep sh' (lgraph_mark_copied g' v' (new_copied_v g to)) v')
+        (graph_rep (lgraph_mark_copied g' v' (new_copied_v g to)))).
+  rewrite <- (lmc_heapgraph_block_ptr g' v' (new_copied_v g to)) in *. subst g'.
+  change (lgraph_mark_copied
+            (lgraph_add_copied_v g v' to) v' (new_copied_v g to))
+    with (lgraph_copy_v g v' to) in *.
+  remember (lgraph_copy_v g v' to) as g'.
+  assert (heapgraph_block_ptr g' v' = heapgraph_block_ptr g v') by
+  (subst g'; apply lcv_heapgraph_block_ptr_old; assumption).
+  assert (heapgraph_block_ptr g' (new_copied_v g to) =
+          heapgraph_block_ptr g (new_copied_v g to)) by
+      (subst g'; apply lcv_heapgraph_block_ptr_new; assumption).
+  assert (writable_share (heapgraph_generation_sh g' (addr_gen v'))) by
+      (unfold heapgraph_generation_sh; apply generation_sh__writable).
+  assert (heapgraph_has_block g' (new_copied_v g to)) by
+      (subst g'; apply lcv_heapgraph_has_block_new; assumption).
+  forward_call (nv).
+  rewrite <- H31 in *.
+  rewrite lacv_heapgraph_block_ptr;
+    [|apply heapgraph_has_block_in_closure|]; try assumption.
+  rewrite <- H32.
+  rewrite <- (lcv_heapgraph_block_ptr g v' to v);
+    try rewrite <- (lcv_heapgraph_block_ptr g v' to v) in H14;
+    try apply heapgraph_has_block_in_closure; try assumption.
+  rewrite (lcv_mfv_Zlen_eq g v v' to H8 H0) in H14. rewrite <- Heqg' in *.
+  remember (heapgraph_generation_sh g' (addr_gen v)) as shh.
+  remember (heapgraph_block_cells_vals g' v) as mfv.
+  remember (new_copied_v g to).
+  remember (labeledgraph_gen_dst g' e a) as g1.
+  assert (0 <= n < Zlength (heapgraph_block_cells_vals g' v)) by
+      (subst g'; rewrite fields_eq_length, <- lcv_block_fields; assumption).
+  assert (Znth n (heapgraph_block_cells g' v) = inr e) by
+      (subst g'; unfold heapgraph_block_cells in *;
+        rewrite <- lcv_block_fields; assumption).
+  assert (0 <= n < Zlength (heapgraph_block_cells g' v)) by
+      (rewrite heapgraph_block_cells_eq_length;
+        rewrite fields_eq_length in H43; assumption).
+  assert (heapgraph_has_block g' v) by
+      (subst g'; apply lcv_heapgraph_has_block_old; assumption).
+  assert (v <> v') by
+      (intro; subst v; clear -v0 H13; lia).
+  assert (block_mark (heapgraph_block g' v) = false) by
+    (subst g'; rewrite <- lcv_block_mark; assumption).
+  assert (writable_share shh) by
+      (rewrite Heqshh; unfold heapgraph_generation_sh; apply generation_sh__writable).
+  localize [vertex_rep (heapgraph_generation_sh g' (addr_gen v)) g' v].
+  unfold vertex_rep, vertex_at. Intros.
+  rewrite Heqmfv in *; rewrite <- Heqshh.
+  forward.
+  rewrite H31.
+  sep_apply (field_at_data_at_cancel
+                shh
+                (tarray int_or_ptr_type (Zlength (heapgraph_block_cells_vals g' v)))
+                (upd_Znth n (heapgraph_block_cells_vals g' v) (heapgraph_block_ptr g' a))
+                (heapgraph_block_ptr g' v)).
+  gather_SEP (data_at shh _ _ _) (data_at shh _ _ _).
+  replace_SEP 0 (vertex_rep (heapgraph_generation_sh g1 (addr_gen v)) g1 v).
+  {
+    unfold vertex_rep, vertex_at.
+    replace (heapgraph_generation_sh g1 (addr_gen v)) with shh by
+        (subst shh g1; reflexivity).
+    replace (Zlength (heapgraph_block_cells_vals g1 v)) with
+        (Zlength (heapgraph_block_cells_vals g' v)) by
+        (subst g1; repeat rewrite fields_eq_length;
+        apply lgd_raw_fld_length_eq).
+    rewrite (lgd_mfv_change_in_one_spot g' v e a n);
+      try assumption. entailer!.
+  }
+  subst g1; subst a.
+  unlocalize [graph_rep (labeledgraph_gen_dst g' e (new_copied_v g to))].
+  {
+    now apply (graph_vertex_lgd_ramif g' v e (new_copied_v g to) n).
+  }
+  remember (new_copied_v g to) as v1.
+  remember (labeledgraph_gen_dst g' e v1) as g1.
+  thaw FR.
+  remember
+    (cut_thread_info t_info (Z.of_nat to) (heapgraph_block_size g v') Hi Hh)
+    as t_info' eqn:Heqt_info'.
+  unfold thread_info_rep. Intros.
+  assert
+    (0 <= 0 < Zlength (ti_args t_info'))
+    by (rewrite arg_size; rep_lia).
+  gather_SEP
+    (data_at _ _ _ _)
+    (heap_struct_rep _ _ _)
+    (heap_rest_rep _).
+  replace_SEP 0 (thread_info_rep sh t_info' ti).
+  {
+    unfold thread_info_rep. simpl heap_head. simpl ti_heap_p.
+    simpl ti_args. simpl ti_heap. entailer!.
+  }
+  rewrite H31 in H33.
+  assert
+    (forward_relation from to 0 (inr e) g g1)
+    by (subst g1 g' v1 v'; constructor; assumption).
+  assert (In e (heapgraph_block_fields g v)).
+  {
+    unfold heapgraph_block_fields.
+    rewrite <- filter_sum_right_In_iff.
+    rewrite <- Heqc.
+    apply (Znth_In n (heapgraph_block_cells g v)).
+    rewrite heapgraph_block_cells_eq_length. assumption.
+  }
+  assert
+    (forward_condition g1 t_info' from to).
+  {
+    subst g1 g' t_info' from v'.
+    assert
+      (heapgraph_has_block (lgraph_copy_v g (dst g e) to) (dst g e))
+      as HH.
+    {
+      destruct H37 ; now constructor.
+    }
+    apply lgd_forward_condition; try assumption.
+    apply lcv_forward_condition_unchanged; try assumption.
+    red.
+    intuition.
+  }
+  remember roots as roots'.
+  assert (super_compatible (g1, t_info', roots') f_info outlier).
+  {
+    subst g1 g' t_info' roots'.
+    apply lgd_super_compatible, lcv_super_compatible_unchanged; try assumption.
+    red; intuition.
+  }
+  assert (thread_info_relation t_info t_info').
+  {
+    subst t_info'. split; [|split]; [reflexivity| |]; intros m.
+    - rewrite cti_gen_size. reflexivity.
+    - rewrite cti_space_base. reflexivity.
+  }
+  forward_if.
+  2: {
+    assert (depth = 0) by lia. subst depth. clear H56.
+    deadvars!. clear Heqnv. forward.
+    Exists g1 t_info' roots. entailer!. simpl. rewrite Heqc.
+    simpl field2forward. rewrite H12. simpl. now constructor.
+  }
+  pose proof H55 as HH55.
+  destruct H55 as [? [? ?]].
+  replace
+    fp
+    with (heapgraph_generation_base g1 from)
+    by (subst fp g1 g'; apply lcv_gen_start; assumption).
+  replace
+    (offset_val fn (heapgraph_generation_base g1 from))
+    with (limit_address g1 t_info' from).
+  2: {
+    subst fn gn.
+    rewrite H57.
+    rewrite <- nth_Znth'.
+    change
+      (nth from (heap_spaces (ti_heap t_info)) default)
+      with (nth_space t_info from).
+    now rewrite (thread_info_relation__space_remembered _ _ _ HH55).
+  }
+  replace
+    n_addr
+    with (next_address t_info' to)
+    by (subst n_addr; rewrite H55; reflexivity).
+  forward_for_simple_bound
+    n'
+    (EX i: Z, EX g3: HeapGraph, EX t_info3: thread_info,
+    PROP (super_compatible (g3, t_info3, roots') f_info outlier;
+          forward_loop
+            from to (Z.to_nat (depth - 1))
+            (sublist 0 i (heapgraph_field_pairs g1 (new_copied_v g to)))
+            g1 g3;
+          forward_condition g3 t_info3 from to;
+          thread_info_relation t_info' t_info3)
+    LOCAL (temp _new nv;
+            temp _sz (if Archi.ptr64 then Vlong (Int64.repr n')
+                      else vint n');
+            temp _from_start (heapgraph_generation_base g3 from);
+            temp _from_limit (limit_address g3 t_info3 from);
+            temp _next (next_address t_info3 to);
+            temp _depth (vint depth))
+    SEP (all_string_constants rsh gv;
+          fun_info_rep rsh f_info fi;
+          outlier_rep outlier;
+          graph_rep g3;
+          thread_info_rep sh t_info3 ti))%assert.
+  {
+    pose proof (block_fields__range2 (heapgraph_block g v')). simpl in H59.
+    now rewrite <- Heqn' in H59.
+  }
+  {
+    Exists g1 t_info'. autorewrite with sublist.
+    assert
+      (forward_loop from to (Z.to_nat (depth - 1)) [] g1 g1)
+      by constructor. unfold thread_info_relation.
+    destruct H54 as [? [? [? ?]]].
+    now entailer!.
+  }
+  - Intros.
+    assert (heapgraph_has_gen g1 to) by
+        (rewrite Heqg1, lgd_graph_has_gen; subst g';
+        rewrite <- lcv_graph_has_gen; assumption).
+    assert (heapgraph_has_block g1 (new_copied_v g to)) by
+      (subst g1; rewrite <- lgd_heapgraph_has_block;
+      rewrite Heqg'; apply lcv_heapgraph_has_block_new; assumption).
+    forward_call (rsh, sh, gv, fi, ti, g3, t_info3, f_info, roots',
+                  outlier, from, to, depth - 1,
+                  (@inr Z _ (new_copied_v g to, i))).
+    + apply prop_right. simpl. rewrite sub_repr.
+        do 4 f_equal. rewrite H31.
+        first [rewrite sem_add_pi_ptr_special' | rewrite sem_add_pl_ptr_special']; auto.
+        * simpl. f_equal.
+          rewrite <- (lgd_heapgraph_block_ptr_eq g' e v1), <- Heqg1.
+          subst v1. apply (fl_heapgraph_block_ptr _ _ _ _ _ _ H64 H61).
+          apply heapgraph_has_block_in_closure; assumption.
+        * rewrite <- H31. assumption.
+    + split3; [| |split].
+        * destruct H53 as [_ [_ [? _]]].
+          apply (fl_heapgraph_has_block _ _ _ _ _ _ H64 H61 _ H65).
+        * erewrite <- fl_block_fields; eauto. subst g1.
+          unfold lgraph_copy_v. subst n'.
+          rewrite <- lgd_raw_fld_length_eq.
+          subst g'. rewrite lcv_vlabel_new.
+          assumption. rewrite v0. lia.
+        * erewrite <- fl_block_mark; eauto. subst g1 from.
+          rewrite <- lgd_block_mark_eq. subst g'.
+          rewrite lcv_vlabel_new; try assumption.
+        * simpl; lia.
+    + Intros vret. destruct vret as [[g4 t_info4] roots4].
+      simpl fst in *. simpl snd in *. Exists g4 t_info4.
+      simpl in H67. subst roots4.
+      assert (heapgraph_generation_base g3 from = heapgraph_generation_base g4 from).
+      {
+        eapply fr_gen_start; eauto.
+        erewrite <- fl_graph_has_gen; eauto.
+      }
+      rewrite H67.
+      assert (limit_address g3 t_info3 from = limit_address g4 t_info4 from).
+      {
+        unfold limit_address. f_equal. 2: assumption. f_equal.
+        rewrite (thread_info_relation__space_remembered _ _ _ H70).
+        destruct H70 as [_ [H71 _]].
+        now rewrite H71.
+      }
+      rewrite H71.
+      assert (next_address t_info3 to = next_address t_info4 to).
+      {
+        unfold next_address. f_equal. destruct H70. assumption.
+      }
+      rewrite H72. clear H67 H71 H72.
+      assert
+        (thread_info_relation t_info' t_info4)
+        by (apply tir_trans with t_info3; assumption).
+      assert
+        (forward_loop
+          from to (Z.to_nat (depth - 1))
+          (sublist 0 (i + 1)
+                  (heapgraph_field_pairs g1 (new_copied_v g to)))
+          g1 g4).
+      {
+        eapply forward_loop_add_tail_vpp; eauto. subst n' g1 from.
+        rewrite <- lgd_raw_fld_length_eq. subst g'.
+        rewrite lcv_vlabel_new; assumption.
+      }
+      entailer!.
+  - Intros g3 t_info3.
+    assert (thread_info_relation t_info t_info3) by
+        (apply tir_trans with t_info';
+        [split; [| split]|]; assumption).
+    rewrite sublist_all in H60.
+    2: { rewrite Z.le_lteq. right. subst n' g1 from.
+        rewrite heapgraph_field_pairs__Zlength,  <- lgd_raw_fld_length_eq.
+        subst g'; rewrite lcv_vlabel_new; auto. }
+    Opaque super_compatible. Exists g3 t_info3 roots.
+    entailer!. simpl.
+    replace (Z.to_nat depth) with (S (Z.to_nat (depth - 1))) by
+        (rewrite <- Z2Nat.inj_succ; [f_equal|]; lia).
+    rewrite Heqc, H12. simpl.
+    constructor; [reflexivity | assumption..].
+    Transparent super_compatible.
+Qed.
